Working on the instr_add proof

src/coq/optimisations/add_instr.v
@@ -11,7 +11,8 @@ Require Import ZArith List String Omega.
 Require Import Vellvm.AstLib Vellvm.Ollvm_ast.
 Require Import Vellvm.optimisations.wellformedSSA.
 Require Import Vellvm.optimisations.EqNat.
-
+Require Import Vellvm.optimisations.transform.
+Require Import Coq.Logic.FunctionalExtensionality.
 From mathcomp.ssreflect
 Require Import ssreflect ssrbool seq eqtype ssrnat fintype.
 
@@ -54,6 +55,12 @@ match b.(blk_term) with
   | (_, _) => Z0
 end.
 
+Definition get_terminator_id (b:block) : instr_id :=
+match b.(blk_term) with
+| (a, _) => a
+end.
+
+
 
 (*Find the largest instruction (which is either the terminator ID or an instruction from within the code) and adds 1 to it*)
 Definition get_first_unused (b:block) : instr_id := IId (Raw (Z.add (get_maximum (get_terminator_iid b) (b.(blk_code))) 1)).
@@ -62,80 +69,48 @@ Definition get_first_unused (b:block) : instr_id := IId (Raw (Z.add (get_maximum
 Definition no_instr : instr := INSTR_Op (SV (VALUE_Null)).
 Print block.
 
-Definition optimise_block (b:block) := mk_block b.(blk_id) b.(blk_phis) (b.(blk_code)++[::(get_first_unused b, no_instr)]) b.(blk_term).
+Definition add_to_block b c :=  mk_block b.(blk_id) b.(blk_phis) (b.(blk_code)++c) b.(blk_term).
+Print block.
+Print terminator.
+Print snd.
+Definition term_check (b:block) : bool :=
+let term := snd b.(blk_term) in
+match term with
+  | TERM_Ret_void => true
+  | _ => false
+end.
 
 
-Print block_to_cmd.
+
+
+Definition optimise_block (b:block) := if (term_check b) then add_to_block b [::(get_first_unused b, no_instr)] else b.
+Definition optimise_program (m:mcfg) := def_cfg_opt optimise_block m.
+
+
 
 
 
 Print find_instr.
 
-(*find_instr = 
-fix find_instr (cd : code) (p t : instr_id) {struct cd} :
-  option (cmd * option instr_id) :=
-  match cd with
-  | [::] => None
-  | (x, i) :: cd0 =>
-      if decide (p = x)
-      then Some (Step i, Some (fallthrough cd0 t))
-      else find_instr cd0 p t
-  end*)
 
+(*END GOAL: find_instr (c ++ d) p t = find_instr_double c d p t*) 
 
-
-Print fallthrough.
-
-(*Some term_id*)
+Lemma instr_id_eq : forall (i1:instr_id), ((i1 == i1) = true).
+Proof. intro.
+Admitted.
 
 
 Definition find_instr_double (c d: code) (p t : instr_id) : option (cmd * option instr_id) :=
 match (find_instr c p t) with
   | None => find_instr d p t
-  | Some (Step i, Some tid ) => if decide (tid = t) then (Some (Step i, Some (fallthrough d t))) else Some (Step i, Some tid)
-  | Some (Step i, None) => None
+  | Some (CFG.Step i, Some tid ) => if decide (tid = t) then (Some (CFG.Step i, Some (fallthrough d t))) else Some (CFG.Step i, Some tid)
+  | Some (CFG.Step i, None) => None
   | Some (Term _, _) => None
 end.
-
-
-
-Lemma remove_nil_r : forall (a: seq (instr_id * instr)), a = a ++ [::].
-Proof. move => //a. induction a. simpl. auto. simpl. rewrite <- IHa. auto. Qed.
-
-Lemma remove_nil_l : forall (a: seq (instr_id * instr)), a = [::] ++ a.
-Proof. move => //a. Qed.
-
-
-Lemma testtest : forall c d p t, find_instr ([::c] ++ d) p t = find_instr_double [::c] d p t.
-Proof. 
-intros. simpl. destruct c. simpl. unfold find_instr_double. simpl. destruct (decide (p = i)). simpl.
-admit. auto. Admitted.
-
-
-Definition test tid t i3 := 
-if eqinstr_id tid t then Some (Step i3, Some t) else Some (Step i3, Some tid).
-
-Lemma foralltest: forall tid t i3, test tid t i3 = Some (Step i3, Some tid). Admitted.
-
-Lemma testtest1 : forall p p0 t, find_instr_double [::p] [::] p0 t = find_instr_double ([::]) ([::p]) p0 t.
-Proof. intros. unfold find_instr_double. simpl. destruct p. simpl. destruct (decide (p0 = i)). simpl. admit. admit.
-Admitted.
-
-Lemma testtest3: forall t, eqinstr_id t t = true.
-Proof. intros. induction t. simpl. admit. admit. Admitted.
-Hint Rewrite testtest3.
-
 
 Lemma not_eq_false : forall (t:instr_id), t <> t -> False.
 Proof. intros. unfold not in H. apply H. auto. Qed.
 
-
-
-Lemma testtest4 : forall c d p t, find_instr ([::c] ++ [::d]) p t = find_instr_double [::c] [::d] p t.
-Proof. intros. induction d, c => //. rewrite /find_instr_double/=. simpl in *. destruct (decide (p = i)). simpl.
-destruct (decide (t = t)). simpl. auto. simpl. assert (t = t) by auto. unfold not in n; apply n in H; inversion H.
-auto.
-Qed.
 
 Lemma testtest5 : forall c d p t, find_instr ([::c] ++ d) p t = find_instr_double [::c] d p t.
 Proof. induction d, c => //.
@@ -149,644 +124,503 @@ destruct (decide (t = t)). simpl. auto. simpl. unfold not in n. assert (t = t) b
 destruct (decide (p = i1)). simpl. auto.
 destruct (decide (p = i3)). simpl in *. auto. auto.
 Qed.
-
-Lemma testtest6 : forall c p t,
-find_instr (c ++ [::]) p t =
-find_instr_double c [::] p t.
-Proof. induction c => //. 
-  + intros. simpl. destruct a. simpl. unfold find_instr_double. simpl. destruct (decide (p = i)).
-simpl. destruct c. simpl. destruct (decide (t = t)).  simpl. auto. simpl. auto. destruct p0. simpl. destruct ((decide (i1 = t))). simpl. subst. auto. simpl. auto.
-simpl. unfold find_instr_double in IHc. simpl in *. auto. Qed.
-
-
-Lemma testtest7 : forall a c p t,
-find_instr ((a::c) ++ [::]) p t =
-find_instr_double (a::c) [::] p t.
-Proof. intros. remember (a :: c) as D. rewrite testtest6. auto. Qed.
-
-
-Definition testfunc1 d p t :=
+Print find_instr.
+Definition helper_func d p t : option (cmd * option instr_id) :=
 match find_instr d p t with
-| Some (Step i7, Some tid) =>
-    if is_left (decide (tid = t)) then Some (Step i7, Some t) else Some (Step i7, Some tid)
-| Some (Step i7, None) => None
+| Some (CFG.Step i7, Some tid) =>
+    if is_left (decide (tid = t)) then Some (CFG.Step i7, Some t) else Some (CFG.Step i7, Some tid)
+| Some (CFG.Step i7, None) => None
 | Some (Term _, _) => None
 | None => None
 end.
 
 
 
-Lemma testtest8: forall d p t, find_instr d p t = testfunc1 d p t.
+Lemma find_instr_eq_helper_func: forall d p t, find_instr d p t = helper_func d p t.
 Proof. induction d => //. intros.
-rewrite testtest5. simpl. unfold testfunc1, find_instr_double. simpl. destruct a. simpl.
+rewrite testtest5. simpl. unfold helper_func, find_instr_double. simpl. destruct a. simpl.
 destruct (decide (p = i)). simpl. destruct (decide (t = t)). simpl.
-induction d. simpl in *. admit. simpl. destruct a. simpl in *. specialize (IHd t). subst.
-admit. simpl. admit.
-admit. Admitted.
+induction d. simpl in *.
+destruct (decide (t = t)); simpl in *; auto.
+simpl. destruct a. simpl in *. specialize (IHd t). subst.
+destruct ((decide (i1 = t))). simpl. subst. auto. simpl. auto.
+assert (t = t) by auto. unfold not in n. apply n in H. inversion H.
+specialize (IHd p t). unfold helper_func in IHd. auto.
+ Qed.
 
-Lemma testtest9 : forall c d p t, p \notin (map fst c) -> p \notin (map fst d) -> find_instr_double c d p t = find_instr_double (c ++ d) [::] p t.
+
+Lemma find_double_eq : forall c d p t,  p \notin (map fst c) ->
+ p \notin (map fst d) -> 
+find_instr_double c d p t = find_instr (c ++ d) p t.
 Proof. induction c, d => //.
-  +unfold find_instr_double. simpl. destruct p. simpl. intros. unfold fallthrough. simpl. destruct d.
-simpl. destruct (decide (p = s)). simpl. admit. admit.
-destruct p0. simpl. induction d. simpl. destruct (decide (p = s)).
-simpl. unfold is_left. simpl. destruct (decide (s0 = t)). simpl. subst. auto.
-destruct (decide (t = t)). simpl. auto. auto.
-simpl. destruct (decide (s0 = t)). subst. destruct (decide (t = t)). auto. auto.
-destruct (decide (s0 = t)). simpl. subst. destruct (decide (t = t)). auto. simpl. unfold negb in H0.
-simpl in *. unfold not in n1. assert (t = t) by auto. apply n1 in H1. inversion H1.
-rewrite e in H0. unfold negb in H0. simpl in *. unfold in_mem in H0. simpl in *. 
-assert ((s == s) = true). admit. rewrite H1 in H0. simpl in H0. inversion H0.
-destruct (decide (p = s0)). simpl. destruct (decide (t = t)). simpl. auto. simpl. auto.
-auto. simpl in *. 
-destruct (decide (p = s)). subst. unfold negb in H0. unfold in_mem in H0. simpl in *.
-assert ((s == s) = true). admit. rewrite H1 in H0. simpl in *. inversion H0.
-simpl in *. simpl in *.
-
-destruct a. simpl in *.
-destruct (decide (p = s0)). simpl in *. subst. unfold negb in H0. unfold in_mem in H0. simpl in *.
-assert ((s0 == s0) = true). admit. rewrite H1 in H0. simpl in *.
-assert ((s0 == s) || true = true).
-destruct ((s0 == s)). simpl. auto. simpl. auto.
-rewrite H2 in H0. inversion H0. simpl.
-
-unfold fallthrough.
-induction d; simpl in *.
-destruct (decide (p = i1)). simpl.
-destruct (decide (t = t)). simpl. auto. simpl. auto. auto.
-simpl in *.
-destruct (decide (p = i1)).
-unfold negb in H0. unfold in_mem in H0. simpl in *.
-subst. 
-assert ((i1 == i1) = true). admit. rewrite H1 in H0. simpl. 
++simpl in *. destruct a. simpl. intros. unfold find_instr_double. simpl. destruct (decide (p = i)).
+subst. unfold negb, in_mem in H; simpl in H. rewrite instr_id_eq in H; simpl in H. inversion H.
+rewrite cats0. induction c. simpl. auto.
+(*by testtest8*)
 admit.
-destruct a. unfold fallthrough in *.
-destruct d.
-destruct (decide (p = i3)).
-admit.
-simpl. auto. destruct p0.
-simpl in *.
-unfold negb in H0. unfold in_mem in H0.
-simpl in*.
-destruct (decide (p = i3)). simpl.
-destruct ((decide (i5 = t))).
-simpl. subst; auto.
-simpl. auto. 
-destruct (decide (p = i5)). simpl. induction d. simpl. admit. admit.
-(*using proof above*)
-admit.
-(*trivial*)
-admit.
-simpl.
+intros. simpl in *.
 
+specialize (IHc (p :: d) p0 t).
+unfold find_instr_double. simpl in *. destruct a. destruct (decide (p0 = i)).
+subst; simpl; unfold negb, in_mem in H; simpl in H. 
+assert ((i == i) = true). admit. rewrite H1 in H. simpl in *. inversion H.
+ simpl in *. unfold find_instr_double in IHc. apply IHc.
+unfold negb in *. admit. auto.
 
-intros. unfold find_instr_double. simpl. 
-destruct a. destruct p. simpl in *. 
-destruct (decide (p0 = s)). simpl in *.
-admit.
-simpl.
+ Admitted.
 
 
-
-induction c. simpl.
-destruct (decide (p0 = s0)). simpl.
-(*trivial*) admit.
-simpl in *.
-(*proof above*) admit.
-simpl. destruct a. simpl in *.
-destruct (decide (p0 = i1)). simpl in *.
-Admitted.
-
-
-
-
-
-
-
-
-
-
-
-
-
-
-
-Lemma testtest8 : forall c d p t, t \notin c -> find_instr (c ++ d) p t = find_instr_double c d p t.
-Proof. induction c, d => //.
-  +intros. rewrite testtest7. auto.
-  +intros. unfold find_instr_double. destruct c. 
-
-
-Lemma remove_nil_r : forall (a: seq instr_id), a = a ++ [::].
-Proof. move => //a. induction a. simpl. auto. simpl. rewrite <- IHa. auto. Qed.
-
-
-Lemma instr_id_comm : forall (a b:instr_id), (a == b) = (b == a).
-Proof. intros. induction a, b => //. Qed.
-
-Lemma uniq_comm_single : forall (a b:instr_id), uniq ([::a] ++ [::b]) = uniq ([::b] ++ [::a]).
-Proof. intros. unfold uniq. simpl. unfold negb. unfold in_mem. simpl. rewrite instr_id_comm. auto.
-Qed.  
-
-
-
-
-Lemma notin_assoc : forall (a b c:instr_id), (a \notin ([::b] ++ [::c])) = ((a \notin [::b]) && (a \notin [::c])).
-Proof. move => //a b c. unfold negb. unfold in_mem. simpl. destruct (a == b) => //; destruct (a == c) => //.
-Qed.
-
-Lemma in_nil : forall (a:instr_id), (a \in [::]) = false.
-Proof. intros. unfold in_mem. simpl. auto. Qed.
-
-
-Lemma in_assoc : forall (a b:instr_id) (c:seq instr_id), (a \in ([::b] ++ c)) = (a \in [::b]) || (a \in c).
-Proof. intros. simpl. induction c => //.
-  +simpl. rewrite in_nil => //. rewrite orb_false_r. auto.
-  +simpl. unfold in_mem in *. simpl in *. destruct ((a == b)). simpl in *. auto.
-simpl in *. destruct ((a == a0)). simpl. auto. simpl. auto. Qed.
-
-
-
-Lemma in_assoc_list : forall (a:instr_id) (b c:seq instr_id), (a \in (b ++ c)) = (a \in b) || (a \in c).
-Proof. move => a b c. induction b, c => //.
-  +simpl. rewrite <- remove_nil_r. rewrite in_nil. rewrite orb_false_r. auto.
-  +simpl in *. unfold in_mem in *. simpl in *. destruct (a == a0) => //. Qed.
-
-
-Lemma in_assoc_r : forall a (b:seq instr_id) i, (i \in b ++ [:: a]) = (i \in b) || (i \in [:: a]).
-Proof. intros. rewrite in_assoc_list. auto. Qed.
-
-
-Lemma notin_assoc_one_list : forall (a b:instr_id) c, (a \notin ([::b] ++ c)) = ((a \notin [::b]) && (a \notin c)).
-Proof. intros. unfold negb. induction c => //.
-  +simpl. rewrite andb_true_r. auto.
-  +simpl in *. unfold in_mem in *. simpl in *. destruct (a == b) => //. Qed.
-
-
-
-Lemma notin : forall (a b:instr_id) (c:seq instr_id), (a \notin ([::b] ++ c) = (a \notin (c ++ [::b]))).
-Proof. intros. unfold negb. simpl. induction c => //.
-  +unfold in_mem. simpl. destruct (a == a0). destruct (a == b). simpl. auto. simpl. auto. rewrite IHc. simpl.
-unfold in_mem. simpl. auto. Qed.
-(*
-Lemma single_in_eq : forall (a i:instr_id), (i \in [:: a]) = (i == a).
-Proof. intros. unfold in_mem. simpl. auto. destruct ((i == a)) => //.
-Qed.
-Lemma testtest : forall (a:instr_id) (b:seq instr_id),  (a \notin b) && uniq b = uniq (b ++ [::a]).
-Proof. move => a b => //. induction b.
-  +simpl. auto.
-  +simpl. rewrite <- IHb. unfold negb. simpl. rewrite in_assoc_r. rewrite in_assoc. simpl.
-rewrite single_in_eq. rewrite single_in_eq. rewrite instr_id_comm. unfold in_mem. remember ((mem b) a) as B.
-destruct b; simpl => //. simpl. destruct (a0 == a). simpl. auto. simpl. auto.
-simpl. destruct (a == i). simpl. destruct (a0 == i). destruct (a0 == a). simpl. auto.
-simpl. auto.
-destruct (a0 == a). destruct (b a0).
-
-
-
-
-Lemma add_instr_preserves_ssa : forall b, well_form_block b -> well_form_block (optimise_block b).
-Proof. move =>// b. constructor. inversion H. unfold unique_instr_id in *. rewrite /optimise_block/=. 
-assert (([seq fst i
-      | i <- blk_code b ++
-             [:: (get_first_unused b, no_instr)]]) = [seq fst i
-      | i <- blk_code b] ++ [::fst (get_first_unused b, no_instr)]) => //. destruct b. simpl in *. induction blk_code => //. simpl.
-apply IHblk_code in H.
-
-
-Admitted.
-
-
-
-*)
-(*
-
-(*The code in a block gets executed sequentially.
-This optimisation adds an instruction to the end of that code therefore the impact this might have is on the block terminator instruction.
-There are currently 4 implemented terminator instructions:
-  | TERM_Ret :  tvalue -> terminator
-  | TERM_Ret_void : terminator
-  | TERM_Br :  tvalue -> block_id -> block_id ->  terminator
-  | TERM_Br_1 : block_id ->  terminator
-
-
-Explanation:
-TERM_Ret - return a typed value
-TERM_Ret_void - return void
-TERM_Br - branch to either block id depending on the evaluation of a typed value
-TERM_Br_1 - branch directly to block_id
-
-
-
-Let's add an instruction to a block if and only if its terminating instruction is TERM_Ret.
-*)
-
-
-
-(*Simple function that returns true if the terminating instruction is a return void*)
-Definition terminator_check (b:block) : bool :=
-match b.(blk_term) with
-  | (_, TERM_Ret_void) => false
-  | _ => false
-end.
-
-
-Definition get_blk_id (b:block) : instr_id :=
-let term := b.(blk_term) in
-match term with 
-  | (term_id, term_instr) => term_id
-end.
-
-Print block.
-
-
-
-Print block_to_cmd.
-Print fallthrough.
-
-
-
-Definition old (c:code) (p:instr_id) (term_id:instr_id) := find_instr c p term_id.
-
-
-Definition add_instr_block (b:block) (i:(instr_id * instr)) (b1:(instr_id * terminator)%type) := 
-mk_block b.(blk_id) b.(blk_phis) (blk_code b ++ (cons i nil)) b1.
-Print blk_term.
-
-Definition get_blk_term (b:block)  :=
-let term := b.(blk_term) in
-match term with 
-  | (term_id, term_instr) => term_instr
-end.
-
-Print block.
-
-
-
-
-
-(*Definition fallthrough (cd: code) term_id : instr_id :=
-  match cd with
-  | [] => term_id
-  | (next, _)::_ => next
-  end.*)
-
-
-
-
-Print block_to_cmd.
-Print find_instr.
-
-
-
-(*
-Definition block_to_cmd (b:block) (iid:instr_id) : option (cmd * option instr_id) :=
+Definition double_block_to_cmd (b:block) (added_code:code) (iid:instr_id) : option (cmd * option instr_id):=
   let term_id := blk_term_id b in 
-  if term_id == iid then
+  if decide (term_id = iid) then
     Some (Term (snd (blk_term b)), None)
   else
-    find_instr (blk_code b) iid term_id 
+    find_instr_double (blk_code b) added_code iid term_id 
 .
 
-
-Fixpoint find_instr (cd : code) (p:instr_id) (t:instr_id) : option (cmd * option instr_id) :=
-  match cd with
-  | [] =>  None
-  | (x,i)::cd =>
-    if p == x then
-      Some (Step i, Some (fallthrough cd t))
-    else
-      find_instr cd p t
-  end.
-
-
-*)
-
-
-Lemma test : forall c d look term, find_instr (c ++ d) look term = find_instr (c ++ d) look term.
-Proof. Admitted.
-
-Definition beq_ascii (a1 a2 : ascii) :=
-  match a1, a2 with
-  | Ascii b1 b2 b3 b4 b5 b6 b7 b8, Ascii c1 c2 c3 c4 c5 c6 c7 c8 =>
-    (eqb b1 c1) && (eqb b2 c2) && (eqb b3 c3) && (eqb b4 c4) &&
-    (eqb b5 c5) && (eqb b6 c6) && (eqb b7 c7) && (eqb b8 c8)
-  end.
-
-
-Fixpoint beq_string (s1 s2 : string) :=
-  match s1, s2 with
-  | EmptyString,  EmptyString  => true
-  | String x1 s1, String x2 s2 => beq_ascii x1 x2 && beq_string s1 s2
-  | _, _                       => false
-  end.
-
-
-Print raw_id.
-Print int.
-Definition beq_raw_id (a b: raw_id) : bool:=
-match a, b with
-  | Name a, Name b => beq_string a b
-  | Anon a, Anon b => Z.eqb a b
-  | Raw a, Raw b => Z.eqb a b
-  | _, _ => false
-end.
-Print instr_id.
-
-
-
-Definition beq_instr_id (a b: instr_id) : bool:=
-match a, b with
-  | IId a, IId b => beq_raw_id a b
-  | IVoid a, IVoid b => Z.eqb a b
-  | _, _ => false
-end.
-
-
-Lemma ascii_eq : forall a, beq_ascii a a = true.
-Proof. intros a. induction a. simpl.
-repeat (rewrite eqb_reflx; simpl). auto. Qed.
-
-Lemma string_eq : forall s, beq_string s s = true.
-Proof. intros. induction s.
-  -simpl. auto.
-  -simpl. rewrite ascii_eq. simpl. rewrite IHs. auto. Qed.
-
-
-
-
-Lemma raw_id_eq : forall a, beq_raw_id a a = true.
-Proof. intros. induction a; simpl; try (rewrite string_eq); try (rewrite Z.eqb_refl); auto.
-Qed.
-
-Lemma instr_id_eq : forall a, beq_instr_id a a = true.
-Proof. intros. induction a; simpl; try (rewrite raw_id_eq); try (rewrite Z.eqb_refl); auto.
-Qed.
-
-Print fallthrough.
-(*Definition fallthrough (cd: code) term_id : instr_id :=
-  match cd with
-  | [] => term_id
-  | (next, _)::_ => next
-  end.*)
-
-
-Definition double_fallthrough (c d: code) (term_id:instr_id) : instr_id :=
-match c with
-  | [] => fallthrough d term_id
-  | _ => fallthrough c term_id
-end.
-
-Lemma double_fallthrough_eq : forall c d term_id, fallthrough (c ++ d) term_id = double_fallthrough c d term_id.
-Proof. intros. unfold double_fallthrough. unfold fallthrough.
-simpl. destruct c; simpl.
-  +simpl. auto.
-  +destruct p. auto.
-Qed.
-
-
-Print block_to_cmd.
-
-
-(*Fixpoint find_instr (cd : code) (p:instr_id) (t:instr_id) : option (cmd * option instr_id) :=
-  match cd with
-  | [] =>  None
-  | (x,i)::cd =>
-    if p == x then
-      Some (Step i, Some (fallthrough cd t))
-    else
-      find_instr cd p t
-  end.*)
-
-
-
-Definition double_find_instr (c d: code) (p :instr_id) (t:instr_id) : option (cmd * option instr_id) :=
-match (find_instr c p t) with
-  | None => (find_instr d p t)
-  | Some (Step i, Some ter) => if beq_instr_id ter t then Some (Step i, Some (fallthrough d t)) else Some (Step i, Some ter)
-  | Some (_, _) => find_instr d p t
-end.
-
-(*
-Lemma help : forall t, (fallthrough [] t) = t.
-Proof. intros. unfold fallthrough; simpl; eauto.
-Qed.
-
-Lemma help1 : forall p t, find_instr [] p t = None.
-Proof. intros. unfold find_instr. auto. Qed.
-
-
-Lemma help2: forall a d p t, find_instr (a::d) p t = double_find_instr (cons a nil) d p t.
-Proof. intros. induction a. simpl. unfold double_find_instr.
-simpl. destruct (p == a ). simpl.
-rewrite instr_id_eq. auto. auto. Qed.
-(* (fallthrough (c ++ d) t))*)
-
-
-
-
-
-Lemma test12 : forall c d p t, find_instr (c ++ d) p t = double_find_instr c d p t.
-Proof. intros.
-unfold double_find_instr. simpl.
-induction c.
-  +simpl. auto.
-  +rewrite help2. 
-assert (((a :: c) ++ d) = cons a (c ++ d)).
-simpl; auto. rewrite H. rewrite help2. 
-unfold double_find_instr. rewrite IHc.
-simpl. destruct a. simpl.
-
-Definition optimise (b:block) := if terminator_check b then (add_instr_block b (get_blk_id b, no_instr) (get_first_unused b, get_blk_term b)) else b.
-
-Definition prog_optimise (p:modul CFG.cfg) := def_cfg_opt optimise p.
-
-(*
-(*V1*)
-(*Get new instructions*)
-
-(*Proof: block_to_cmd (optimise b) p = fetch_two_block b (optimise b) (new:code) p*)
-
-
-
-Definition fetch_two_block_full  (b:block) (p:instr_id) :=
-if terminator_check b then (fetch_two_block b (optimisev1 b) (cons (get_first_unused b, no_instr) nil) p) else (block_to_cmd b p).
-
-
-Lemma block_eq : forall b p, block_to_cmd (optimisev1 b) p = fetch_two_block_full b p.
-Proof. intros. unfold block_to_cmd. unfold fetch_two_block_full. unfold optimisev1. 
-unfold terminator_check. destruct b. simpl. destruct blk_term. simpl. unfold blk_term_id. 
-unfold block_to_cmd. simpl. unfold fetch_two_block. simpl. unfold blk_term_id. simpl.
-destruct t; simpl; auto.
-  +unfold block_to_cmd. simpl. unfold blk_term_id. simpl. unfold get_first_unused. simpl.
-destruct (i == p). auto.
-  *destruct blk_code. simpl. unfold get_terminator_iid. simpl. unfold not in n.
-induction i; simpl; auto. induction id. simpl.
-
-Require Import Vellvm.optimisations.transform. 
-
-
-Definition optimise_addv1 (b:block) := if terminator_check b then cons (get_first_unused b, no_instr) nil else nil.
-
-Definition prog_optimisev1 (p:modul CFG.cfg) := def_cfg_opt optimisev1 p.
-
-
-(*In the proof, there will always be the case:
-  fetch prog pc = ...
-  fetch (optimise prog) pc = ...
-
-As seen in the pacoproof.v, it is useful to write (fetch (optimise prog) pc) as a new function of fetch prog pc.
-This allows us to 
-*)
-(*V2*)(*
-Definition optimisev2 (b:block) := if terminator_check b then (add_instr_block b (get_blk_id b, no_instr) (
-*)
-Print block_to_cmd.
-
-
-
-
-Print find_instr.
-Print block_to_cmd.
-
-
-
-(**************************************************************************)
-Definition dual_block_to_cmd (b:block) (i:instr_id) := if terminator_check b then fetch_two_block b (cons (get_first_unused b, no_instr) nil) i else block_to_cmd b i .
-
-
-Require Import Vellvm.Classes.
-Definition dual_fetch (CFG: mcfg) (p:pc) :=
+Definition double_block_to_cmd_check b added_code iid :=
+if (term_check b) then double_block_to_cmd b added_code iid else block_to_cmd b iid.
+
+Lemma double_block_to_cmd_eq : forall b iid, block_to_cmd (optimise_block b) iid = double_block_to_cmd_check b [::(get_first_unused b, no_instr)] iid.
+Proof. destruct b. unfold block_to_cmd. simpl.
+unfold double_block_to_cmd_check. simpl. unfold double_block_to_cmd. simpl.
+unfold optimise_block. simpl. unfold term_check. simpl. destruct blk_term.
+simpl. induction t.
+  +simpl. unfold block_to_cmd. simpl. unfold blk_term_id. simpl. auto.
+  +simpl. unfold block_to_cmd. intros. unfold blk_term_id. simpl.
+assert
+
+
+(find_instr_double blk_code
+    [:: (get_first_unused
+           {|
+           blk_id := blk_id;
+           blk_phis := blk_phis;
+           blk_code := blk_code;
+           blk_term := (i, TERM_Ret_void) |}, no_instr)] iid 
+    i
+
+
+=
+
+(find_instr
+    (blk_code ++
+     [:: (get_first_unused
+            {|
+            blk_id := blk_id;
+            blk_phis := blk_phis;
+            blk_code := blk_code;
+            blk_term := (i, TERM_Ret_void) |}, no_instr)]) iid 
+    i)). apply find_double_eq. admit. admit. rewrite H. 
+destruct (decide (i = iid)); simpl; auto.
+
+  +simpl. unfold block_to_cmd. simpl. unfold blk_term_id. simpl. auto.
+  +simpl. unfold block_to_cmd. simpl. unfold blk_term_id. simpl. auto.
+  +simpl. unfold block_to_cmd. simpl. unfold blk_term_id. simpl. auto.
+  +simpl. unfold block_to_cmd. simpl. unfold blk_term_id. simpl. auto.
+  +simpl. unfold block_to_cmd. simpl. unfold blk_term_id. simpl. auto.
+  +simpl. unfold block_to_cmd. simpl. unfold blk_term_id. simpl. auto.
+Admitted.
+
+
+Definition double_fetch (CFG : mcfg) (p:pc) : option cmd :=
   let 'mk_pc fid bid iid := p in 
   'cfg <- find_function CFG fid;
   'blk <- find_block (blks (df_instrs cfg)) bid;
-  '(c, _) <- dual_block_to_cmd blk iid;
+  '(c, _) <- double_block_to_cmd_check blk [::(get_first_unused blk, no_instr)] iid;
   mret c.
 
 
 
-Lemma test1 : forall b i, dual_block_to_cmd b i = block_to_cmd (optimisev1 b) i.
-Proof. intros. unfold dual_block_to_cmd. unfold terminator_check.
-destruct b. simpl. unfold optimisev1. simpl. unfold get_first_unused. simpl. destruct blk_term.
-simpl. destruct t; simpl; auto.
-  -unfold fetch_two_block. simpl. unfold block_to_cmd. simpl. unfold blk_term_id.
-simpl. unfold get_terminator_iid. simpl. destruct (i0 == i); auto.
-induction blk_code. simpl. auto.
-remember (i ==
-    IId
-      (Raw
-         (match i0 with
-          | IId (Name _) => 0
-          | IId (Anon _) => 0
-          | IId (Raw n0) => n0
-          | IVoid _ => 0
-          end + 1)%Z)) as A. destruct A; auto. simpl. destruct a. simpl.
-destruct (i == i1). simpl. unfold fallthrough. simpl.
-destruct blk_code. simpl. unfold not in n. destruct i1. simpl. destruct id. simpl.
-destruct i0. destruct id; simpl. simpl in *.
-Qed.
+Definition test1 a (bk:block_id) pt :=
+match find_block (blks (df_instrs a)) bk with
+    | Some a0 =>
+        match block_to_cmd a0 pt with
+        | Some (c, _) => Some c
+        | None => None
+        end
+    | None => None
+    end.
 
 
-
-Print fetch.
-
-
-Definition fetch1 (CFG : mcfg) (p:pc) : option cmd :=
-  let 'mk_pc fid bid iid := p in 
-  'cfg <- find_function CFG fid;
-  'blk <- find_block (blks (df_instrs cfg)) bid;
-  '(c, _) <- dual_block_to_cmd blk iid;
-  mret c.
-
-
-
-
-
-Lemma equal_fetch : forall m p, fetch (prog_optimisev1 m) p = fetch1 m p.
-Proof. intros.
-destruct m. simpl.
-induction m_definitions.
-  +unfold prog_optimisev1 in *. unfold optimisev1. simpl. unfold def_cfg_opt. simpl. unfold fetch, fetch1. simpl. auto.
-  +simpl in *. unfold fetch, fetch1 in *. simpl. destruct p. simpl in *. destruct a. simpl in *.
-unfold find_function in *. simpl in *. unfold find_defn in *. simpl in *.
-unfold cfg_opt in *. simpl in *. auto. unfold ident_of in *. simpl in *. 
-unfold ident_of_definition in *. unfold ident_of in *. simpl in *.
-
-destruct (ident_of_declaration df_prototype == ID_Global fn).
-    *simpl in *. destruct df_instrs. simpl in *. induction blks; simpl in *; auto.
-      -destruct a. simpl. unfold optimisev1. simpl. unfold terminator_check. simpl.
-{destruct blk_term. simpl. destruct t; simpl; destruct (blk_id == bk); try (rewrite test1; unfold optimisev1; simpl; auto);
-try (induction blks; simpl; auto).
-}
-    *auto.
-Qed.
-
-
-
+Definition test2 a bk pt :=
+  match find_block (blks (df_instrs a)) bk with
+    | Some a0 =>
+        match double_block_to_cmd_check a0 [:: (get_first_unused a0, no_instr)] pt with
+        | Some (c, _) => Some c
+        | None => None
+        end
+    | None => None
+    end.
 Print find_block.
 
-(******************SECOND*************************)
+Lemma testeq : forall a bk pt, test1 (cfg_opt optimise_block a) bk pt = test2 a bk pt.
+Proof.
+destruct a. simpl. unfold test1, test2.
+simpl. destruct df_instrs. simpl. induction blks.
++simpl. auto.
++simpl. intros.
 
 
 
-Definition incr_pc1 (CFG : mcfg) (p:pc) : option pc :=
+destruct a. simpl. destruct blk_term. simpl; induction t; simpl; destruct (decide (blk_id = bk)); try rewrite <- double_block_to_cmd_eq; auto.
+
+
+
+  +admit.
+  +admit.
+  +admit.
+  +admit.
+  +admit.
+  +admit.
+  +admit.
+Admitted.
+
+
+ (* destruct a. destruct df_instrs. induction blks => //.
+unfold test1, test2. simpl.
+
+
+
+
+
+
+
+
+
+ destruct df_instrs. induction blks => //.
+intros. unfold test1, test2. simpl. destruct (decide (blk_id a = bk)).
+
+
+assert (block_to_cmd (optimise_block a) pt = double_block_to_cmd_check a [:: (get_first_unused a, no_instr)] pt).
+apply double_block_to_cmd_eq. rewrite H. auto.
+
+simpl in *. unfold test1, test2 in IHblks. simpl in *.
+simpl. specialize (IHblks bk pt). 
+
+
+assert ( List.find (fun b : block => if decide (blk_id b = bk) then true else false)
+    (List.map optimise_block blks) = 
+find_block (List.map optimise_block blks) bk).
+destruct blks. simpl. auto. simpl.
+destruct (decide (blk_id b = bk)). simpl. auto. simpl. f_equal.
+apply functional_extensionality. intros. destruct (decide (blk_id x = bk)) => //.
+unfold is_left in H. simpl in *. destruct blks. simpl in *. auto.
+simpl in *. apply IHblks. Qed.*) 
+
+
+Definition test1_v1 mcfg fn bk pt :=
+match find_function mcfg fn with
+| Some a => test1 a bk pt
+| None => None
+end.
+
+Definition test2_v1 mcfg fn bk pt :=
+match find_function mcfg fn with
+| Some a => test2 a bk pt
+| None => None
+end.
+
+
+
+Lemma testeq_v1 : forall mcfg fn bk pt, test1_v1 (optimise_program mcfg) fn bk pt = test2_v1 mcfg fn bk pt.
+Proof. intros. unfold test1_v1. simpl. unfold test2_v1.
+destruct mcfg. induction m_definitions.
+  +simpl. auto.
+  +unfold find_function. simpl. unfold find_defn. simpl.
+unfold cfg_opt. simpl. unfold alter_blocks. simpl. unfold ident_of. simpl. unfold ident_of_definition. simpl.
+destruct (decide (ident_of (df_prototype a) = ID_Global fn)). simpl.
+rewrite testeq. auto.
+simpl.
+unfold find_function in *. simpl in *.
+unfold find_defn in *. simpl in *. rewrite IHm_definitions. auto.
+Qed.
+
+
+Lemma double_fetch_eq : forall m p, fetch (optimise_program m) p = double_fetch m p.
+Proof. intros. unfold double_fetch. unfold fetch. simpl.
+destruct p. simpl.
+destruct m. simpl. induction m_definitions. simpl. auto.
+unfold find_function. simpl. unfold find_defn. unfold ident_of.
+simpl. unfold ident_of_definition. simpl.
+destruct (decide (ident_of (df_prototype a) = ID_Global fn)). simpl.
+destruct a. simpl. destruct df_instrs. simpl. induction blks.
+simpl. auto.
+simpl.  unfold optimise_block. simpl. destruct a. simpl. unfold term_check.
+
+destruct blk_term. simpl.
+destruct t.
+
+  +simpl in *. destruct (decide (blk_id = bk) ). simpl. rewrite <- double_block_to_cmd_eq. auto. admit.
+  +simpl in *. destruct (decide (blk_id = bk)). simpl in *. rewrite <- double_block_to_cmd_eq. auto. admit.
+  +simpl in *. destruct (decide (blk_id = bk)). simpl in *. rewrite <- double_block_to_cmd_eq. auto. admit.
+  +simpl in *. destruct (decide (blk_id = bk)). simpl in *. rewrite <- double_block_to_cmd_eq. auto. admit.
+  +simpl in *. destruct (decide (blk_id = bk)). simpl in *. rewrite <- double_block_to_cmd_eq. auto. admit.
+  +simpl in *. destruct (decide (blk_id = bk)). simpl in *. rewrite <- double_block_to_cmd_eq. auto. admit.
+  +simpl in *. destruct (decide (blk_id = bk)). simpl in *. rewrite <- double_block_to_cmd_eq. auto. admit.
+  +simpl in *. destruct (decide (blk_id = bk)). simpl in *. rewrite <- double_block_to_cmd_eq. auto. admit.
+(*
+simpl.
+
+
+unfold find_function in *. simpl in *.
+
+assert (Util.find_map (find_defn fn)
+                      (List.map (cfg_opt optimise_block) m_definitions)
+= Util.find_map
+    (fun d : definition cfg =>
+     if decide (ident_of (df_prototype d) = ID_Global fn)
+     then Some d
+     else None) (List.map (cfg_opt optimise_block) m_definitions)).
+simpl. unfold find_defn. f_equal. apply functional_extensionality.
+intros. unfold is_left. simpl.
+unfold ident_of. unfold ident_of_definition. unfold ident_of.
+destruct (decide (ident_of_declaration (df_prototype x) = ID_Global fn)); auto.
+
+
+
+
+
+
+
+
+
+rewrite H in IHm_definitions.
+
+
+
+
+assert (Util.find_map (find_defn fn) m_definitions
+=
+(Util.find_map
+    (fun d : definition cfg =>
+     if decide (ident_of (df_prototype d) = ID_Global fn)
+     then Some d
+     else None) m_definitions)).
+
+unfold find_defn. unfold is_left.
+f_equal.
+apply functional_extensionality. intros.
+unfold ident_of. unfold ident_of_definition.
+unfold ident_of.
+destruct (decide (ident_of_declaration (df_prototype x) = ID_Global fn)); simpl; eauto.
+rewrite H0 in IHm_definitions.
+
+induction m_definitions.
+simpl in *. auto. 
+assert (match find_function (optimise_program m) fn with
+| Some a =>
+    match find_block (blks (df_instrs a)) bk with
+    | Some a0 =>
+        match block_to_cmd a0 pt with
+        | Some (c, _) => Some c
+        | None => None
+        end
+    | None => None
+    end
+| None => None
+end = test1_v1 (optimise_program m) fn bk pt) by auto.
+assert (match find_function m fn with
+| Some a =>
+    match find_block (blks (df_instrs a)) bk with
+    | Some a0 =>
+        match
+          double_block_to_cmd a0 [:: (get_first_unused a0, no_instr)] pt
+        with
+        | Some (c, _) => Some c
+        | None => None
+        end
+    | None => None
+    end
+| None => None
+end = test2_v1 m fn bk pt) by auto.
+rewrite H; rewrite H0. apply testeq_v1.  *) Admitted.
+
+(*********************************)
+
+
+
+
+
+Definition double_incr_pc (CFG:mcfg) (p:pc) : option pc :=
   let 'mk_pc fid bid iid := p in 
   'cfg <- find_function CFG fid;
   'blk <- find_block (blks (df_instrs cfg)) bid;
-  '(c, n) <- dual_block_to_cmd blk iid;
+  '(c, n) <- double_block_to_cmd_check blk [::(get_first_unused blk, no_instr)] iid;
   'iid_next <- n;
   mret (mk_pc fid bid iid_next).
 
-Lemma equal_incr_pc : forall m p, incr_pc (prog_optimisev1 m) p = incr_pc1 m p.
-Proof. intros. destruct m. simpl.
-destruct m_definitions; simpl in *.
-  +unfold prog_optimisev1 in *. unfold optimisev1. simpl. unfold def_cfg_opt. simpl. unfold incr_pc, incr_pc1. simpl. auto.
-  +simpl in *. unfold incr_pc, incr_pc1 in *. simpl. destruct p. simpl in *. destruct d. simpl in *.
-unfold find_function in *. simpl in *. unfold find_defn in *. simpl in *.
-unfold cfg_opt in *. simpl in *. auto. unfold ident_of in *. simpl in *. 
-unfold ident_of_definition in *. unfold ident_of in *. simpl in *.
 
-destruct (ident_of_declaration df_prototype == ID_Global fn).
-    *simpl in *. destruct df_instrs. simpl in *. induction blks.
-      -simpl in *. auto.
-      -destruct a. simpl. unfold optimisev1. simpl. unfold terminator_check. simpl.
-{destruct blk_term. simpl. destruct t; simpl; destruct (blk_id ==bk); try (rewrite test1; unfold optimisev1; simpl; eauto); try (induction blks; simpl; eauto).
-}
-    *induction m_definitions.
-      -simpl. auto.
-      -simpl.
-{destruct (ident_of_declaration (Ollvm_ast.df_prototype a) == ID_Global fn).
-        +simpl. destruct a. simpl in *. induction df_instrs0. 
-          -simpl in *. induction blks.
-            *simpl. auto.
-            *simpl. unfold optimisev1. unfold terminator_check. simpl. destruct a. simpl in *. destruct blk_term. clear IHm_definitions. simpl in *.
-{destruct t; simpl; destruct (blk_id == bk);
-try (simpl; unfold dual_block_to_cmd, block_to_cmd, blk_term_id; simpl; auto);
-try (induction blks; simpl; auto; auto).
-unfold fetch_two_block. simpl.
-unfold block_to_cmd; simpl in *.
-unfold blk_term_id; simpl in *.
-  *destruct (i == pt); auto. induction blk_code.
-    -simpl. unfold get_blk_id. simpl. induction (pt == i); auto.
-    -simpl. destruct a. destruct (pt == i0). simpl.
-unfold get_blk_id; simpl in *.
-unfold fallthrough. simpl. induction blk_code. simpl.
-auto.
-auto.
-auto.
-  *clear IHblks. clear IHblks0. 
-unfold fetch_two_block. simpl. unfold block_to_cmd. simpl.
-unfold get_blk_id. simpl. unfold blk_term_id. simpl.
-subst.
-destruct (i == pt); auto.
-induction blk_code; auto.
-  +simpl. destruct (pt == i); auto.
-  +simpl. destruct a0. destruct (pt == i0); auto. unfold fallthrough. 
-simpl. destruct blk_code; simpl; auto.
-}
-  +auto.
-}
-Qed.*)
 
-*)*)
-*)
-(**************************************************************************)
+
+Definition test3_v1 a bk pt fn := 
+match find_block (blks (df_instrs a)) bk with
+    | Some a0 =>
+        match block_to_cmd a0 pt with
+        | Some (_, Some a2) =>
+            Some {| fn := fn; bk := bk; pt := a2 |}
+        | Some (_, None) => None
+        | None => None
+        end
+    | None => None
+    end
+.
+
+Definition test4_v1 a bk pt fn  :=
+match find_block (blks (df_instrs a)) bk with
+    | Some a0 =>
+        match
+          double_block_to_cmd a0
+            [:: (get_first_unused a0, no_instr)] pt
+        with
+        | Some (_, Some a2) =>
+            Some {| fn := fn; bk := bk; pt := a2 |}
+        | Some (_, None) => None
+        | None => None
+        end
+    | None => None
+    end
+.
+
+
+
+
+Lemma test_eq2 : forall a bk pt fn, test3_v1 (cfg_opt optimise_block a) bk pt fn = test4_v1 a bk pt fn.
+Proof. intros. (*
+destruct a. destruct df_instrs. simpl. induction blks.
+  +unfold test3_v1, test4_v1. simpl. auto.
+  +unfold test3_v1, test4_v1 in *. simpl in *.
+destruct (decide (blk_id a = bk)). rewrite double_block_to_cmd_eq. auto.
+simpl in *.
+assert ( find_block (List.map optimise_block blks) bk =
+  List.find
+    (fun b : block =>
+     if decide (blk_id b = bk) then true else false)
+    (List.map optimise_block blks)).
+destruct blks; simpl; auto. destruct (decide (blk_id b = bk)); simpl; auto.
+f_equal. apply functional_extensionality. intros. destruct (decide (blk_id x = bk)); simpl; auto.
+rewrite H in IHblks.
+assert (find_block blks bk =   List.find
+    (fun b : block =>
+     if decide (blk_id b = bk) then true else false) blks).
+destruct blks; simpl; auto. destruct (decide (blk_id b = bk)); simpl; auto. f_equal.
+apply functional_extensionality. intros. destruct (decide (blk_id x = bk)); simpl; auto.
+rewrite H0 in IHblks. simpl in *.
+induction blks. simpl in *. auto. simpl in *.
+destruct (decide (blk_id a0 = bk)). simpl in *. auto.
+ simpl in *. rewrite H0. rewrite H. apply IHblks. *) Admitted.
+
+
+
+Definition test3_v2 m bk pt fn :=
+match find_function m fn with
+| Some a => test3_v1 a bk pt fn
+| None => None
+end.
+
+
+Definition test4_v2 m bk pt fn :=
+match find_function m fn with
+| Some a => test4_v1 a bk pt fn
+| None => None
+end.
+
+
+
+Lemma test_eq3 : forall mcfg fn bk pt, test3_v2 (optimise_program mcfg) fn bk pt = test4_v2 mcfg fn bk pt.
+Proof. intros. unfold test3_v2, test4_v2. destruct mcfg. induction m_definitions.
+  +simpl. auto.
+  +unfold find_function; simpl in *.  unfold find_defn. simpl. unfold ident_of.
+simpl. unfold ident_of_definition. simpl.
+destruct (decide (ident_of (df_prototype a) = ID_Global pt)). rewrite test_eq2. auto.
+simpl.
+unfold find_function in *. simpl. unfold find_defn in *. simpl in *.
+rewrite IHm_definitions. auto. Qed.
+
+
+
+
+
+
+Lemma double_incr_pc_eq : forall m p, incr_pc (optimise_program m) p = double_incr_pc m p.
+Proof. intros. destruct p. simpl.
+assert (match find_function (optimise_program m) fn with
+| Some a =>
+    match find_block (blks (df_instrs a)) bk with
+    | Some a0 =>
+        match block_to_cmd a0 pt with
+        | Some (_, Some a2) =>
+            Some {| fn := fn; bk := bk; pt := a2 |}
+        | Some (_, None) => None
+        | None => None
+        end
+    | None => None
+    end
+| None => None
+end = test3_v2 (optimise_program m) bk pt fn). unfold test3_v2. unfold test3_v1.
+auto. rewrite H. clear H.
+
+assert (match find_function m fn with
+| Some a =>
+    match find_block (blks (df_instrs a)) bk with
+    | Some a0 =>
+        match
+          double_block_to_cmd a0
+            [:: (get_first_unused a0, no_instr)] pt
+        with
+        | Some (_, Some a2) =>
+            Some {| fn := fn; bk := bk; pt := a2 |}
+        | Some (_, None) => None
+        | None => None
+        end
+    | None => None
+    end
+| None => None
+end = test4_v2 m bk pt fn). unfold test4_v2. unfold test4_v1. simpl.
+Admitted.
+
+
+
+(**************)
+(*Jump equiv*)
+
+
+
+Print jump.
+Locate jump.
+Print find_block.
+
+Definition jump_test1 a function_id end_bid:=
+      match find_block (blks (df_instrs a)) end_bid with
+      | Some a0 => Some (block_to_entry function_id a0)
+      | None => None
+      end
+.
+Print jump_test1.
+
+Print find_block.
+
+
+Definition jump_test2 a function_id end_bid :=
+      match find_block (blks (df_instrs a)) end_bid with
+      | Some a0 => Some (block_to_entry function_id (optimise_block a0))
+      | None => None
+      end.
+Print jump_test1.
+
+
+Lemma jump_test_eq : forall mcfg function_id end_bid, jump_test1 (cfg_opt optimise_block mcfg) function_id end_bid = jump_test2 mcfg function_id end_bid.
+Proof. intros. unfold jump_test1, jump_test2. simpl. destruct mcfg. simpl. destruct df_instrs. simpl.
+induction blks. simpl. auto.
+simpl. unfold optimise_block. simpl. unfold blk_id. simpl. destruct a. simpl.
+
+unfold term_check. simpl. destruct blk_term. simpl. destruct t.
+destruct (decide (blk_id = end_bid)). simpl. auto. admit.
+simpl. destruct (decide (blk_id = end_bid)). simpl. auto. admit.
+destruct (decide (blk_id = end_bid)). simpl. auto. admit.
+destruct (decide (blk_id = end_bid)). simpl. auto. admit.
+destruct (decide (blk_id = end_bid)). simpl. auto. admit.
+destruct (decide (blk_id = end_bid)). simpl. auto. admit.
+destruct (decide (blk_id = end_bid)). simpl. auto. admit.
+destruct (decide (blk_id = end_bid)). simpl. auto. admit.
+Admitted.
