src/coq/optimisations/add_instrproof.v
@@ -1,14 +1,15 @@
 
 Require Import ZArith List String Omega.
 Require Import  Vellvm.Ollvm_ast Vellvm.Classes Vellvm.Util Vellvm.CFGProp Vellvm.CFG.
-
+Require Import Vellvm.optimisations.wellformedSSA.
 Require Import Vellvm.optimisations.transform.
 Require Import Vellvm.optimisations.add_instr.
 Require Import paco.
 Require Import Vellvm.Memory.
 Require Import Vellvm.Effects.
+From mathcomp.ssreflect
+Require Import ssreflect ssrbool seq eqtype ssrnat.
 
-(*
 Print find_function.
 
 
@@ -39,16 +40,9 @@ Essentially, we want to solve this by induction on the terminator instruction of
 
 Print incr_pc.
 
-
-Inductive pc_match : mcfg -> pc -> (mcfg -> mcfg) -> pc -> Prop :=
-  | match_pc_intro : forall m p i j k l f, incr_pc m p = Some l -> incr_pc (f m) p = Some k -> fetch m p = Some i  -> fetch (f m) p = Some j -> pc_match m p f p.
-
 Print state.
-Inductive state_match : mcfg -> (mcfg -> mcfg) -> state -> state -> Prop :=
-  | match_state_intro : forall m f p e s, pc_match m p f p -> state_match m f (p, e, s) (p, e, s).
 
-
-Ltac try_finish X := simpl; try (simpl; constructor; constructor; auto); try ( constructor; right; apply X).
+Ltac try_finish := simpl; try (simpl; constructor; constructor; auto).
 
 Print fetch.
 
@@ -60,40 +54,1601 @@ match fetch m p with
   | None => None
 end.
 
-Print prog_optimise.
-Print optimise.
-
-Print prog_optimise.
-Print def_cfg_opt.
 
 Definition nothing o : block := o.
-
+Print find_instr.
 
 Definition prog_nothing := def_cfg_opt nothing.
 
-Lemma add_instrproof : (forall st st1 prog, state_match prog prog_optimise st st1) -> forall st prog mem, trace_equiv (memD mem (sem ((def_cfg_opt nothing) prog) st)) (memD mem (sem (prog) st)).
-Proof. intro. pcofix CIH. Admitted.
+
+Ltac finish X :=
+repeat match goal with
+  | [ |- trace_equiv_step (upaco2 (trace_equiv_step (X:=())) _) (Vis (trace_map (fun _ : state => ()) <$> Err _)) (Vis (trace_map (fun _ : state => ()) <$> Err _)) ] => constructor; constructor
+  | [ |- related_event_step (upaco2 (trace_equiv_step (X:=())) _) (Vis (trace_map (fun _ : state => ()) <$> Err _)) (Vis (trace_map (fun _ : state => ()) <$> Err _)) ] => constructor
+  | [ |- trace_equiv_step (upaco2 (trace_equiv_step (X:=())) _) (Vis (trace_map (fun _ : state => ()) <$> Fin _)) (Vis (trace_map (fun _ : state => ()) <$> Fin _)) ] => constructor; constructor; auto
+  | [ |- trace_equiv_step (upaco2 (trace_equiv_step (X:=())) _) (Tau () (memD _ (trace_map (fun _ : state => ()) (step_sem _ _)))) (Tau () (memD _ (trace_map (fun _ : state => ()) (step_sem _ _))))] => constructor; right; apply X
+
+end.
+
+Ltac destr_simpl P X:= destruct P; simpl in *; finish X.
+
+Print terminator.
+
+Print pc.
+
+
+
+
+
+Lemma add_instrproof : (forall m fn bk pt, well_formed_program m optimise_program fn bk pt) -> (forall (t:terminator), t = TERM_Ret_void) -> forall st prog mem, trace_equiv (memD mem (sem (optimise_program prog) st)) (memD mem (sem (prog) st)).
+Proof. intros PROGRAM CHECK. pcofix CIH. intros. pfold.
+destruct st.
+destruct p.
+
+
+
+
+
+assert (memD mem (sem prog (p, e, s)) = unroll (memD mem (sem prog (p, e, s)))).
+destruct (memD mem (sem prog (p, e, s))); simpl; auto. rewrite H. clear H.
+
+assert ((memD mem (sem (optimise_program prog) (p, e, s))) = unroll ((memD mem (sem (optimise_program prog) (p, e, s))))).
+destruct ((memD mem (sem (optimise_program prog) (p, e, s)))); simpl; auto. rewrite H. clear H.
+
+simpl.
+
+
+rewrite double_fetch_eq.
+rewrite double_incr_pc_eq.
+
+destruct p.
+unfold double_fetch. simpl. unfold double_block_to_cmd_check. unfold double_block_to_cmd.
+simpl. unfold find_instr_double. simpl.
+unfold block_to_cmd.
+
+
+
+
+
+remember (find_function prog fn) as A.
+destr_simpl A CIH.
+destr_simpl d CIH.
+destr_simpl df_instrs CIH. simpl in *.
+remember (find_block blks bk) as B.
+destr_simpl B CIH.
+
+unfold term_check.
+destr_simpl b CIH. simpl in *.
+destr_simpl blk_term CIH.
+
+
+generalize (CHECK t). intros.
+unfold blk_term_id. simpl.
+destr_simpl t CIH; try inversion H.
+unfold is_left. simpl in *.
+destr_simpl (decide (i = pt)) CIH; subst.
+destr_simpl s CIH.
+destr_simpl f CIH.
+
+remember (find_instr blk_code pt i) as C.
+destr_simpl C CIH.
+destr_simpl p CIH.
+destr_simpl c CIH.
+destr_simpl o CIH.
+destr_simpl (decide (i1 = i)) CIH; subst.
+destr_simpl pt CIH.
+destr_simpl i0 CIH.
+
+
+destr_simpl (eval_op e None op) CIH. simpl.
+
+
+
+
+
+(*FIRST SIMULATION*)
+
+constructor. left.
+remember (({|
+            fn := fn;
+            bk := bk;
+            pt := get_first_unused
+                    {|
+                    blk_id := blk_id;
+                    blk_phis := blk_phis;
+                    blk_code := blk_code;
+                    blk_term := (i, TERM_Ret_void) |} |}, 
+           add_env id v e, s)) as NEW_STATE.
+
+assert ((memD mem
+     (trace_map (fun _ : state => ())
+        (step_sem prog
+           ({| fn := fn; bk := bk; pt := i |}, add_env id v e, s)))) = unroll (memD mem
+     (trace_map (fun _ : state => ())
+        (step_sem prog
+           ({| fn := fn; bk := bk; pt := i |}, add_env id v e, s))))).
+destruct (memD mem
+     (trace_map (fun _ : state => ())
+        (step_sem prog
+           ({| fn := fn; bk := bk; pt := i |}, add_env id v e, s)))); auto.
+rewrite H0. clear H0.
+
+assert ((memD mem
+     (trace_map (fun _ : state => ())
+        (step_sem (optimise_program prog) NEW_STATE))) = unroll (memD mem
+     (trace_map (fun _ : state => ())
+        (step_sem (optimise_program prog) NEW_STATE)))).
+destruct (memD mem
+     (trace_map (fun _ : state => ())
+        (step_sem (optimise_program prog) NEW_STATE))); auto.
+rewrite H0. clear H0. pfold.
+simpl.
+
+
+(*term in old*)
+rewrite <- HeqA. simpl.
+rewrite <- HeqB. simpl.
+unfold block_to_cmd. unfold blk_term_id. simpl.
+unfold stepD.
+subst.
+
+
+rewrite double_incr_pc_eq.
+rewrite double_fetch_eq.
+unfold double_fetch. simpl.
+rewrite <- HeqA. simpl.
+rewrite <- HeqB. simpl.
+unfold double_block_to_cmd_check.
+
+unfold term_check. unfold  blk_term. simpl.
+unfold double_block_to_cmd. simpl.
+unfold blk_term_id. simpl.
+unfold is_left.
+unfold find_instr_double.
+
+
+simpl.
+
+
+destr_simpl (decide
+                      (i =
+                       get_first_unused
+                         {|
+                         blk_id := blk_id;
+                         blk_phis := blk_phis;
+                         blk_code := blk_code;
+                         blk_term := (i, TERM_Ret_void) |})) CIH.
+
+
+(*wrong, i = (i + 1)*) admit.
+
+unfold not in n0.
+
+remember (find_instr blk_code
+                   (get_first_unused
+                      {|
+                      blk_id := blk_id;
+                      blk_phis := blk_phis;
+                      blk_code := blk_code;
+                      blk_term := (i, TERM_Ret_void) |}) i) as D.
+
+destr_simpl D CIH. (*wrong?*) admit.
+
+
+simpl.
+
+
+destruct (decide
+                   (get_first_unused
+                      {|
+                      blk_id := blk_id;
+                      blk_phis := blk_phis;
+                      blk_code := blk_code;
+                      blk_term := (i, TERM_Ret_void) |} =
+                    get_first_unused
+                      {|
+                      blk_id := blk_id;
+                      blk_phis := blk_phis;
+                      blk_code := blk_code;
+                      blk_term := (i, TERM_Ret_void) |})).
+
++simpl.
+
+
+constructor. 
+
+remember ((step_sem (optimise_program prog)
+           ({| fn := fn; bk := bk; pt := i |},
+           add_env
+             (Raw
+                (get_maximum
+                   (get_terminator_iid
+                      {|
+                      blk_id := blk_id;
+                      blk_phis := blk_phis;
+                      blk_code := blk_code;
+                      blk_term := (i, TERM_Ret_void) |}) blk_code + 1)%Z)
+             (DV VALUE_Null) (add_env id v e), s))) as NEWSTATE.
+
+assert ((memD mem (trace_map (fun _ : state => ()) NEWSTATE)) = unroll (memD mem (trace_map (fun _ : state => ()) NEWSTATE))).
+destruct (memD mem (trace_map (fun _ : state => ()) NEWSTATE)); auto. rewrite H0. simpl. subst. clear H0.
+unfold step_sem. unfold stepD.
+rewrite double_incr_pc_eq.
+rewrite double_fetch_eq.
+unfold double_fetch.
+unfold double_incr_pc.
+simpl. rewrite <- HeqA. simpl. rewrite <- HeqB.
+unfold double_block_to_cmd_check.
+unfold term_check. simpl.
+unfold double_block_to_cmd.
+unfold blk_term_id. unfold blk_term. simpl.
+unfold is_left.
+
+
+destruct (decide (i = i)); simpl.
+
+
+
+destr_simpl s CIH.
+destr_simpl f CIH.
+constructor. right. apply CIH.
+
+
+
+
+unfold not in n1.
+assert (i = i) by auto.
+apply n1 in H0. inversion H0.
+
+
+simpl. (* no instruction on left*) admit.
+
+
+(*****************)
+
+
+destr_simpl fn0 CIH.
+destr_simpl i0 CIH.
+
+
+admit.
+
+
+(*SECOND SIMULATION*)
+
+
+constructor. left.
+
+
+remember ({| fn := fn; bk := bk; pt := i |},
+           add_env id (DVALUE_Addr (Datatypes.length mem)) e, s) as NEWSTATE.
+
+
+assert   ((memD (mem ++ [:: undef])%list
+     (trace_map (fun _ : state => ()) (step_sem prog NEWSTATE))) = unroll
+  (memD (mem ++ [:: undef])%list
+     (trace_map (fun _ : state => ()) (step_sem prog NEWSTATE)))).
+destruct   (memD (mem ++ [:: undef])%list
+     (trace_map (fun _ : state => ()) (step_sem prog NEWSTATE))); auto.
+rewrite H0. simpl. clear H0. subst. unfold stepD.
+unfold fetch. unfold incr_pc.
+unfold block_to_cmd. simpl. rewrite <- HeqA; simpl.
+
+rewrite <- HeqB; simpl. unfold blk_term_id. unfold blk_term.
+simpl.
+
+
+
+(*LEFT DONE*)
+
+
+
+
+
+remember ({|
+            fn := fn;
+            bk := bk;
+            pt := get_first_unused
+                    {|
+                    blk_id := blk_id;
+                    blk_phis := blk_phis;
+                    blk_code := blk_code;
+                    blk_term := (i, TERM_Ret_void) |} |},
+           add_env id (DVALUE_Addr (Datatypes.length mem)) e, s) as NEWSTATE.
+
+
+assert ((memD (mem ++ [:: undef])%list
+     (trace_map (fun _ : state => ())
+        (step_sem (optimise_program prog) NEWSTATE))) = unroll (memD (mem ++ [:: undef])%list
+     (trace_map (fun _ : state => ())
+        (step_sem (optimise_program prog) NEWSTATE)))).
+destruct (memD (mem ++ [:: undef])%list
+     (trace_map (fun _ : state => ())
+        (step_sem (optimise_program prog) NEWSTATE))); auto.
+rewrite H0. simpl. subst.
+clear H0.
+unfold stepD.
+
+rewrite double_incr_pc_eq.
+rewrite double_fetch_eq.
+unfold double_fetch.
+unfold double_incr_pc.
+simpl. rewrite <- HeqA. simpl. rewrite <- HeqB.
+unfold double_block_to_cmd_check.
+unfold term_check. simpl.
+unfold double_block_to_cmd.
+unfold blk_term_id. unfold blk_term. simpl.
+unfold is_left.
+
+
+destruct (decide
+                    (i =
+                     get_first_unused
+                       {|
+                       blk_id := blk_id;
+                       blk_phis := blk_phis;
+                       blk_code := blk_code;
+                       blk_term := (i, TERM_Ret_void) |})); simpl.
+
+(*i != i + 1*) admit.
+
+unfold find_instr_double. simpl.
+
+destruct (find_instr blk_code
+                   (get_first_unused
+                      {|
+                      blk_id := blk_id;
+                      blk_phis := blk_phis;
+                      blk_code := blk_code;
+                      blk_term := (i, TERM_Ret_void) |}) i).
+
+(*find_instr blk_code of get_first_unused should give None*) admit.
+destruct (                 decide
+                   (get_first_unused
+                      {|
+                      blk_id := blk_id;
+                      blk_phis := blk_phis;
+                      blk_code := blk_code;
+                      blk_term := (i, TERM_Ret_void) |} =
+                    get_first_unused
+                      {|
+                      blk_id := blk_id;
+                      blk_phis := blk_phis;
+                      blk_code := blk_code;
+                      blk_term := (i, TERM_Ret_void) |})). simpl.
+pfold. 
+constructor.
+
+
+
+
+
+remember ({| fn := fn; bk := bk; pt := i |},
+           add_env
+             (Raw
+                (get_maximum
+                   (get_terminator_iid
+                      {|
+                      blk_id := blk_id;
+                      blk_phis := blk_phis;
+                      blk_code := blk_code;
+                      blk_term := (i, TERM_Ret_void) |}) blk_code + 1)%Z)
+             (DV VALUE_Null)
+             (add_env id (DVALUE_Addr (Datatypes.length mem)) e), s) as NEWSTATE.
+
+
+assert (  (memD (mem ++ [:: undef])%list
+     (trace_map (fun _ : state => ())
+        (step_sem (optimise_program prog) NEWSTATE))) = unroll   (memD (mem ++ [:: undef])%list
+     (trace_map (fun _ : state => ())
+        (step_sem (optimise_program prog) NEWSTATE)))).
+destruct (  (memD (mem ++ [:: undef])%list
+     (trace_map (fun _ : state => ())
+        (step_sem (optimise_program prog) NEWSTATE)))); auto.
+rewrite H0. simpl. clear H0.
+subst.
+
+unfold stepD.
+
+
+rewrite double_incr_pc_eq.
+rewrite double_fetch_eq.
+unfold double_fetch.
+unfold double_incr_pc.
+simpl. rewrite <- HeqA. simpl. rewrite <- HeqB.
+unfold double_block_to_cmd_check.
+unfold term_check. simpl.
+unfold double_block_to_cmd.
+unfold blk_term_id. unfold blk_term. simpl.
+unfold is_left.
+
+
+destruct (decide (i = i)).
+simpl. destr_simpl s CIH.
+destr_simpl f CIH.
+unfold not in n1. assert ( i = i) by auto.
+apply n1 in H0. inversion H0.
+simpl. (*no instruction on the right*) admit.
+
+
+(*****************)
+
+
+
+destr_simpl ptr CIH.
+destr_simpl (eval_op e (Some t0) v) CIH.
+destr_simpl v0 CIH.
+
+
+
+
+
+
+
+(*THIRD SIMULATION*)
+
+
+
+constructor. left.
+
+
+remember ({| fn := fn; bk := bk; pt := i |},
+           add_env id ((List.nth_default undef mem a)) e, s) as NEWSTATE.
+
+
+assert   ( (memD mem (trace_map (fun _ : state => ()) (step_sem prog NEWSTATE))) = unroll
+  ( (memD mem (trace_map (fun _ : state => ()) (step_sem prog NEWSTATE))))).
+
+
+
+
+
+
+
+
+destruct   ( (memD mem (trace_map (fun _ : state => ()) (step_sem prog NEWSTATE)))); auto.
+rewrite H0. simpl. clear H0. subst. unfold stepD.
+unfold fetch. unfold incr_pc.
+unfold block_to_cmd. simpl. rewrite <- HeqA; simpl.
+
+rewrite <- HeqB; simpl. unfold blk_term_id. unfold blk_term.
+simpl.
+
+
+
+
+
+
+
+
+(*LEFT DONE*)
+
+
+
+
+
+remember (({|
+            fn := fn;
+            bk := bk;
+            pt := get_first_unused
+                    {|
+                    blk_id := blk_id;
+                    blk_phis := blk_phis;
+                    blk_code := blk_code;
+                    blk_term := (i, TERM_Ret_void) |} |},
+           add_env id (List.nth_default undef mem a) e, s)) as NEWSTATE.
+
+
+assert ((memD mem
+     (trace_map (fun _ : state => ())
+        (step_sem (optimise_program prog) NEWSTATE))) = unroll (memD mem
+     (trace_map (fun _ : state => ())
+        (step_sem (optimise_program prog) NEWSTATE)))).
+destruct (memD mem
+     (trace_map (fun _ : state => ())
+        (step_sem (optimise_program prog) NEWSTATE))); auto.
+rewrite H0. simpl. subst.
+clear H0.
+unfold stepD.
+
+rewrite double_incr_pc_eq.
+rewrite double_fetch_eq.
+unfold double_fetch.
+unfold double_incr_pc.
+simpl. rewrite <- HeqA. simpl. rewrite <- HeqB.
+unfold double_block_to_cmd_check.
+unfold term_check. simpl.
+unfold double_block_to_cmd.
+unfold blk_term_id. unfold blk_term. simpl.
+unfold is_left.
+
+
+destruct (decide
+                    (i =
+                     get_first_unused
+                       {|
+                       blk_id := blk_id;
+                       blk_phis := blk_phis;
+                       blk_code := blk_code;
+                       blk_term := (i, TERM_Ret_void) |})); simpl.
+
+
+(*i != i + 1*) admit.
+
+unfold find_instr_double. simpl.
+
+destruct (find_instr blk_code
+                   (get_first_unused
+                      {|
+                      blk_id := blk_id;
+                      blk_phis := blk_phis;
+                      blk_code := blk_code;
+                      blk_term := (i, TERM_Ret_void) |}) i).
+
+(*find_instr blk_code of get_first_unused should give None*) admit.
+destruct (                 decide
+                   (get_first_unused
+                      {|
+                      blk_id := blk_id;
+                      blk_phis := blk_phis;
+                      blk_code := blk_code;
+                      blk_term := (i, TERM_Ret_void) |} =
+                    get_first_unused
+                      {|
+                      blk_id := blk_id;
+                      blk_phis := blk_phis;
+                      blk_code := blk_code;
+                      blk_term := (i, TERM_Ret_void) |})). simpl.
+pfold. 
+constructor.
+
+
+
+
+
+remember ({| fn := fn; bk := bk; pt := i |},
+           add_env
+             (Raw
+                (get_maximum
+                   (get_terminator_iid
+                      {|
+                      blk_id := blk_id;
+                      blk_phis := blk_phis;
+                      blk_code := blk_code;
+                      blk_term := (i, TERM_Ret_void) |}) blk_code + 1)%Z)
+             (DV VALUE_Null) (add_env id (List.nth_default undef mem a) e),
+           s) as NEWSTATE.
+
+
+assert (  (memD mem
+     (trace_map (fun _ : state => ())
+        (step_sem (optimise_program prog) NEWSTATE))) = unroll (memD mem
+     (trace_map (fun _ : state => ())
+        (step_sem (optimise_program prog) NEWSTATE)))).
+destruct (memD mem
+  (trace_map (fun _ : state => ())
+     (step_sem (optimise_program prog) NEWSTATE))); auto.
+rewrite H0. simpl. clear H0.
+subst.
+
+unfold stepD.
+
+
+rewrite double_incr_pc_eq.
+rewrite double_fetch_eq.
+unfold double_fetch.
+unfold double_incr_pc.
+simpl. rewrite <- HeqA. simpl. rewrite <- HeqB.
+unfold double_block_to_cmd_check.
+unfold term_check. simpl.
+unfold double_block_to_cmd.
+unfold blk_term_id. unfold blk_term. simpl.
+unfold is_left.
+
+
+destruct (decide (i = i)).
+simpl. destr_simpl s CIH.
+destr_simpl f CIH.
+unfold not in n1. assert ( i = i) by auto.
+apply n1 in H0. inversion H0.
+simpl. (*no instruction on the right*) admit.
+
+
+
+(*****************)
+
+
+
+destr_simpl i0 CIH.
+destr_simpl fn0 CIH.
+destr_simpl i0 CIH.
+
+
+(*JUMP*) admit.
+
+
+destr_simpl val CIH.
+destr_simpl ptr CIH.
+destr_simpl (eval_op e (Some t) v) CIH;
+destr_simpl (eval_op e (Some t0) v0) CIH.
+
+destr_simpl v2 CIH.
+
+
+
+(*FOURTH SIMULATION*)
+
+
+
+
+constructor. left.
+
+
+remember ({|
+            fn := fn;
+            bk := bk;
+            pt := get_first_unused
+                    {|
+                    blk_id := blk_id;
+                    blk_phis := blk_phis;
+                    blk_code := blk_code;
+                    blk_term := (i, TERM_Ret_void) |} |}, e, s) as NEWSTATE.
+
+
+assert   ( ((memD (replace mem a v1)
+     (trace_map (fun _ : state => ())
+        (step_sem prog ({| fn := fn; bk := bk; pt := i |}, e, s))))) = unroll
+  ( (memD (replace mem a v1)
+     (trace_map (fun _ : state => ())
+        (step_sem prog ({| fn := fn; bk := bk; pt := i |}, e, s)))))).
+
+
+
+
+
+
+
+
+destruct   ( (memD (replace mem a v1)
+     (trace_map (fun _ : state => ())
+        (step_sem prog ({| fn := fn; bk := bk; pt := i |}, e, s))))); auto.
+
+
+rewrite H0. simpl. clear H0. subst. unfold stepD.
+unfold fetch. unfold incr_pc.
+unfold block_to_cmd. simpl. rewrite <- HeqA; simpl.
+
+rewrite <- HeqB; simpl. unfold blk_term_id. unfold blk_term.
+simpl.
+
+
+
+
+
+
+
+
+(*LEFT DONE*)
+
+
+
+
+
+remember (({|
+            fn := fn;
+            bk := bk;
+            pt := get_first_unused
+                    {|
+                    blk_id := blk_id;
+                    blk_phis := blk_phis;
+                    blk_code := blk_code;
+                    blk_term := (i, TERM_Ret_void) |} |}, e, s)) as NEWSTATE.
+
+
+assert ((memD (replace mem a v1)
+     (trace_map (fun _ : state => ())
+        (step_sem (optimise_program prog) NEWSTATE))) = unroll (memD (replace mem a v1)
+     (trace_map (fun _ : state => ())
+        (step_sem (optimise_program prog) NEWSTATE)))).
+destruct (memD (replace mem a v1)
+     (trace_map (fun _ : state => ())
+        (step_sem (optimise_program prog) NEWSTATE))); auto.
+rewrite H0. simpl. subst.
+clear H0.
+unfold stepD.
+
+rewrite double_incr_pc_eq.
+rewrite double_fetch_eq.
+unfold double_fetch.
+unfold double_incr_pc.
+simpl. rewrite <- HeqA. simpl. rewrite <- HeqB.
+unfold double_block_to_cmd_check.
+unfold term_check. simpl.
+unfold double_block_to_cmd.
+unfold blk_term_id. unfold blk_term. simpl.
+unfold is_left.
+
+
+destruct (decide
+                    (i =
+                     get_first_unused
+                       {|
+                       blk_id := blk_id;
+                       blk_phis := blk_phis;
+                       blk_code := blk_code;
+                       blk_term := (i, TERM_Ret_void) |})); simpl.
+
+
+(*i != i + 1*) admit.
+
+unfold find_instr_double. simpl.
+
+destruct (find_instr blk_code
+                   (get_first_unused
+                      {|
+                      blk_id := blk_id;
+                      blk_phis := blk_phis;
+                      blk_code := blk_code;
+                      blk_term := (i, TERM_Ret_void) |}) i).
+
+(*find_instr blk_code of get_first_unused should give None*) admit.
+destruct (                 decide
+                   (get_first_unused
+                      {|
+                      blk_id := blk_id;
+                      blk_phis := blk_phis;
+                      blk_code := blk_code;
+                      blk_term := (i, TERM_Ret_void) |} =
+                    get_first_unused
+                      {|
+                      blk_id := blk_id;
+                      blk_phis := blk_phis;
+                      blk_code := blk_code;
+                      blk_term := (i, TERM_Ret_void) |})). simpl.
+pfold. 
+constructor.
+
+
+
+
+
+remember ({| fn := fn; bk := bk; pt := i |},
+           add_env
+             (Raw
+                (get_maximum
+                   (get_terminator_iid
+                      {|
+                      blk_id := blk_id;
+                      blk_phis := blk_phis;
+                      blk_code := blk_code;
+                      blk_term := (i, TERM_Ret_void) |}) blk_code + 1)%Z)
+             (DV VALUE_Null) e, s) as NEWSTATE.
+
+
+assert (  (memD (replace mem a v1)
+     (trace_map (fun _ : state => ())
+        (step_sem (optimise_program prog) NEWSTATE))) = unroll (memD (replace mem a v1)
+     (trace_map (fun _ : state => ())
+        (step_sem (optimise_program prog) NEWSTATE)))).
+destruct (memD (replace mem a v1)
+  (trace_map (fun _ : state => ())
+     (step_sem (optimise_program prog) NEWSTATE))); auto.
+rewrite H0. simpl. clear H0.
+subst.
+
+unfold stepD.
+
+
+rewrite double_incr_pc_eq.
+rewrite double_fetch_eq.
+unfold double_fetch.
+unfold double_incr_pc.
+simpl. rewrite <- HeqA. simpl. rewrite <- HeqB.
+unfold double_block_to_cmd_check.
+unfold term_check. simpl.
+unfold double_block_to_cmd.
+unfold blk_term_id. unfold blk_term. simpl.
+unfold is_left.
+
+
+destruct (decide (i = i)).
+simpl. destr_simpl s CIH.
+destr_simpl f CIH.
+unfold not in n1. assert ( i = i) by auto.
+apply n2 in H0. inversion H0.
+simpl. (*no instruction on the right*) admit.
+
+
+
+(*****************)
+
+destr_simpl pt CIH.
+destr_simpl i0 CIH.
+
+destr_simpl (eval_op e None op) CIH.
+destr_simpl fn0 CIH.
+
+destr_simpl i0 CIH.
+
+
+(*JUMP*) admit.
+
+destr_simpl ptr CIH.
+
+
+destr_simpl (eval_op e (Some t0) v) CIH.
+destr_simpl v0 CIH.
+destr_simpl i0 CIH.
+destr_simpl fn0 CIH.
+destr_simpl i0 CIH.
+
+
+
+
+(*JUMP*) admit.
+
+
+destr_simpl val CIH.
+destr_simpl ptr CIH.
+destr_simpl (eval_op e (Some t) v) CIH;
+destr_simpl (eval_op e (Some t0) v0) CIH.
+destr_simpl v2 CIH.
+
+(*No instruction on right*?*)
+admit.
+
+(*No instruction on the left? *)
+admit.
+
+
+Admitted.
+
+
+
+
+
+(*Below was past experiments*)
+
+
+
+
+
+
 (*
 
-intros. pfold. generalize (H st st prog). intros. 
-inversion H0. simpl. subst. inversion H1. simpl. subst.
 
-assert ((memD mem (sem (def_cfg_opt nothing prog) (p, e, s))) = unroll ((memD mem (sem (def_cfg_opt nothing prog) (p, e, s))))).
-destruct ((memD mem (sem (def_cfg_opt nothing prog) (p, e, s)))); eauto.
-rewrite H6.
+ destr_simpl b0 CIH.
+destr_simpl blk_term CIH.
+generalize (CHECK t). intros.
+destr_simpl t CIH; try inversion H0.
+  +unfold block_to_cmd. unfold blk_term_id. simpl in *. destr_simpl (decide (i = pt)) CIH; subst.
+destr_simpl s CIH.
+destr_simpl f CIH.
 
-assert ((memD mem (sem prog (p, e, s))) = unroll (memD mem (sem prog (p, e, s)))
-). destruct (memD mem (sem prog (p, e, s))); eauto.
 
-rewrite H6. rewrite H7. clear H6; clear H7. simpl.
 
-destruct prog; simpl in *.
-unfold def_cfg_opt. simpl.
-induction m_definitions.
-  +unfold fetch in *; simpl in *. destruct p. inversion H4.
-  +unfold fetch in *. simpl in *. destruct p. simpl in *.
-unfold find_function in *. simpl in *.
-unfold find_defn in *.
-unfold cfg_opt in *; simpl in *.
-unfold AstLib.ident_of in *; simpl in *.
-*)*)
+
+
+
+
+
+
+
+
+
+
+
+
+
+
+
+
+
+
+
+
+
+
+
+
+
+
+destr_simpl s CIH. destr_simpl f CIH.
+destr_simpl (find_instr blk_code pt i) CIH. destr_simpl p CIH.
+destr_simpl c CIH. destr_simpl o CIH. destr_simpl (decide (i1 = i)) CIH; subst.
+destr_simpl pt CIH. destr_simpl i0 CIH.
+destr_simpl (eval_op e None op) CIH.
+
+(*
+
+
+
+
+ destr_simpl (find_instr blk_code pt i) CIH.
+destr_simpl p CIH. destr_simpl c CIH. destr_simpl o CIH.
+destr_simpl (i1 == i) CIH; subst. destr_simpl pt CIH.
+destr_simpl i0 CIH. destr_simpl (eval_op e None op) CIH.
+        -(*SIMULATION*) admit.
+    *destr_simpl fn0 CIH. destr_simpl i0 CIH.
+        -(*JUMP*) admit.
+        -(*SIMULATION*) admit.
+    *destr_simpl ptr CIH. destr_simpl (eval_op e (Some t0) v) CIH.
+destr_simpl v0 CIH.
+        -(*SIMULATION*) admit.
+    *destr_simpl i0 CIH. destr_simpl fn0 CIH. destr_simpl i0 CIH.
+        -(*JUMP*) admit.
+    *destr_simpl val CIH; destr_simpl ptr CIH. destr_simpl (eval_op e (Some t) v) CIH; destr_simpl (eval_op e (Some t0) v0) CIH.
+destr_simpl v2 CIH.
+        -(*SIMULATION*) admit.
+    *destr_simpl pt CIH. destr_simpl i0 CIH. destr_simpl (eval_op e None op) CIH.
+destr_simpl fn0 CIH. destr_simpl i0 CIH.
+        -(*JUMP*) admit.
+    *destr_simpl ptr CIH. destr_simpl (eval_op e (Some t0) v) CIH.
+destr_simpl v0 CIH. destr_simpl i0 CIH. destr_simpl fn0 CIH.
+destr_simpl i0 CIH.
+        -(*JUMP*) admit.
+    *destr_simpl val CIH; destr_simpl ptr CIH. destr_simpl (eval_op e (Some t) v) CIH; destr_simpl (eval_op e (Some t0) v0) CIH.
+destruct v2; simpl. constructor; constructor. constructor; constructor. constructor; right; apply CIH. constructor; constructor.
+constructor; constructor. constructor; constructor. constructor; constructor.
+generalize (CHECK t); intros. induction t; try inversion H0.
+Admitted. 
+(*
+(*TERM_RET*)
+  +unfold block_to_cmd. unfold blk_term_id. simpl. destr_simpl (i == pt) CIH. destr_simpl v CIH.
+destr_simpl (eval_op e (Some t) v) CIH. destr_simpl s CIH.
+destr_simpl f CIH. destr_simpl (find_instr blk_code pt i) CIH.
+destr_simpl p CIH. destr_simpl c CIH. destr_simpl o CIH.
+destr_simpl pt CIH. destr_simpl i0 CIH. destr_simpl (eval_op e None op) CIH.
+destr_simpl fn0 CIH. destr_simpl i0 CIH. admit.
+destr_simpl ptr CIH. destr_simpl (eval_op e (Some t0) v0) CIH.
+destr_simpl v1 CIH. destr_simpl i0 CIH. destr_simpl fn0 CIH.
+destr_simpl i0 CIH. admit.
+
+destr_simpl val CIH; destr_simpl ptr CIH.
+destr_simpl (eval_op e (Some t) v0) CIH;
+destr_simpl (eval_op e (Some t0) v1) CIH.
+destr_simpl v3 CIH.
+destr_simpl t CIH.
+destr_simpl v0 CIH.
+destr_simpl (eval_op e (Some t) v0) CIH.
+destr_simpl s CIH.
+destr_simpl f CIH.
+destr_simpl s CIH.
+destr_simpl f CIH.
+destr_simpl v0 CIH.
+destr_simpl (eval_op e (Some t) v0) CIH.
+destr_simpl v1 CIH.
+destr_simpl (StepSemantics.Int1.eq x StepSemantics.Int1.one) CIH.
+admit.
+admit.
+admit.
+
+
+
+
+
+
+
+  +unfold block_to_cmd. unfold blk_term_id. simpl.
+destr_simpl (i == pt ) CIH.
+destr_simpl s CIH.
+destr_simpl f CIH.
+destr_simpl (find_instr blk_code pt i) CIH.
+destr_simpl p CIH.
+destr_simpl c CIH.
+destr_simpl o CIH.
+destr_simpl (i1 == i) CIH; subst.
+  *destr_simpl pt CIH. destr_simpl i0 CIH. destr_simpl (eval_op e None op) CIH.
+    -remember ((memD mem (trace_map (fun _ : state => ()) (step_sem prog ({| fn := fn; bk := bk; pt := i |}, add_env id v e, s))))) as A.
+remember ((memD mem (trace_map (fun _ : state => ()) (step_sem (optimise_program prog) ({|  fn := fn;  bk := bk; pt := get_first_unused
+{| blk_id := blk_id;  blk_phis := blk_phis;  blk_code := blk_code; blk_term := (i,  TERM_Ret_void) |} |}, add_env id v e, s))))) as B.
+constructor. left. pfold.
+assert (A = unroll A). destruct A; auto.
+rewrite H. clear H.
+assert (B = unroll B). destruct B; auto. rewrite H. clear H.
+subst. simpl.
+
+remember (             match find_function (optimise_program prog) fn with
+             | Some a =>
+                 match find_block (CFG.blks (df_instrs a)) bk with
+                 | Some a0 =>
+                     match
+                       block_to_cmd a0
+                         (get_first_unused
+                            {|
+                            blk_id := blk_id;
+                            blk_phis := blk_phis;
+                            blk_code := blk_code;
+                            blk_term := (i, TERM_Ret_void) |})
+                     with
+                     | Some (c, _) => Some c
+                     | None => None
+                     end
+                 | None => None
+                 end
+             | None => None
+             end) as A.
+assert (A = double_fetch prog (mk_pc fn bk i)). admit.
+rewrite H. clear HeqA. subst.
+
+remember (                 match find_function (optimise_program prog) fn with
+                 | Some a =>
+                     match find_block (CFG.blks (df_instrs a)) bk with
+                     | Some a0 =>
+                         match
+                           block_to_cmd a0
+                             (get_first_unused
+                                {|
+                                blk_id := blk_id;
+                                blk_phis := blk_phis;
+                                blk_code := blk_code;
+                                blk_term := (i, TERM_Ret_void) |})
+                         with
+                         | Some (_, Some a2) => Some {| fn := fn; bk := bk; pt := a2 |}
+                         | Some (_, None) => None
+                         | None => None
+                         end
+                     | None => None
+                     end
+                 | None => None
+                 end) as B.
+assert (B = double_incr_pc prog (mk_pc fn bk i)). admit.
+clear HeqB. subst.
+unfold double_fetch, double_incr_pc. simpl.
+unfold double_block_to_cmd_check.
+
+
+
+
+
+
+
+
+
+
+
+
+    -destr_simpl fn0 CIH. destr_simpl i0 CIH. admit. (*simulation 2*) admit.
+destr_simpl ptr CIH. destr_simpl (eval_op e (Some t0) v) CIH. destr_simpl v0 CIH.
+(*simulation 3*) admit. destr_simpl i0 CIH. destr_simpl fn0 CIH.
+destr_simpl i0 CIH. admit. destr_simpl val CIH; destr_simpl ptr CIH.
+destr_simpl (eval_op e (Some t) v) CIH;
+destr_simpl (eval_op e (Some t0) v0) CIH.
+destr_simpl v2 CIH.
+(*simulation 4*) admit.
+*destr_simpl pt CIH.
+destr_simpl i0 CIH.
+destr_simpl (eval_op e None op) CIH.
+destr_simpl fn0 CIH.
+destr_simpl i0 CIH.
+admit.
+destr_simpl ptr CIH. destr_simpl (eval_op e (Some t0) v) CIH.
+destr_simpl v0 CIH.
+destr_simpl i0 CIH.
+destr_simpl fn0 CIH.
+destr_simpl i0 CIH.
+admit.
+destr_simpl val CIH; destr_simpl ptr CIH.
+destr_simpl (eval_op e (Some t) v) CIH;
+destr_simpl (eval_op e (Some t0) v0) CIH.
+destr_simpl v2 CIH.
+admit.
+admit.
+
+
++admit.
++admit.
++admit.
++admit.
++admit.
++admit.
+(*
+
+
+
+
+
+
+
+
+
+
+    *(*First simulation*) admit.
+
+
+
+
+
+
+
+
+
+
+
+
+
+
+
+    *destr_simpl fn0 (CIH). destr_simpl i0 CIH. admit.
+
+    *destr_simpl ptr CIH. destr_simpl (eval_op e (Some t0) v0) CIH.
+    *destr_simpl v1 CIH. admit.
+    *destr_simpl i0 CIH. destr_simpl fn0 CIH. destr_simpl i0 CIH. admit. 
+destr_simpl val CIH. destr_simpl ptr CIH. destr_simpl (eval_op e (Some t) v0) CIH.
+destr_simpl (eval_op e (Some t0) v1) CIH. destr_simpl v3 CIH. admit.
+destr_simpl pt CIH. destr_simpl i0 CIH. destr_simpl (eval_op e None op) CIH.
+destr_simpl fn0 CIH. destr_simpl i0 CIH. admit.
+destr_simpl ptr CIH. destr_simpl (eval_op e (Some t0) v0) CIH.
+destr_simpl v1 CIH. destr_simpl i0 CIH. destr_simpl fn0 CIH.
+destr_simpl i0 CIH. admit. destr_simpl val CIH; destr_simpl ptr CIH.
+destr_simpl (eval_op e (Some t) v0) CIH; destr_simpl (eval_op e (Some t0) v1) CIH.
+destr_simpl v3 CIH. destr_simpl t CIH.
+destr_simpl v0 CIH. destr_simpl (eval_op e (Some t) v0) CIH.
+destr_simpl s CIH. destr_simpl f CIH. destr_simpl s CIH. destr_simpl f CIH.
+destr_simpl v0 CIH. destr_simpl (eval_op e (Some t) v0) CIH.
+destr_simpl v1 CIH. destr_simpl (StepSemantics.Int1.eq x StepSemantics.Int1.one) CIH.
+admit. admit. admit.
+
+
+
+
+Admitted.
+(*
+
+
+
+
+rewrite double_fetch_eq. 
+rewrite double_incr_pc_eq.
+
+destruct p.
+
+
+inversion wff_prog. subst.
+inversion wff_optimised_prog. subst.
+inversion block_wf.
+inversion block_wf0.
+
+
+unfold double_fetch. simpl.
+unfold double_block_to_cmd_check.
+unfold double_block_to_cmd. simpl.
+
+
+rewrite function_find0.
+
+
+
+destruct p.
+unfold double_fetch. unfold double_incr_pc.
+simpl.
+unfold fetch. 
+unfold incr_pc.
+
+unfold double_block_to_cmd_check. unfold double_block_to_cmd.
+unfold find_instr_double. simpl.
+unfold block_to_cmd. simpl. unfold find_function. simpl.
+destruct (find_map (find_defn fn) m_definitions). simpl. destruct d.
+simpl. destruct df_instrs. simpl. destruct (find_block blks bk).
+simpl. destruct b. 
+simpl. unfold term_check. simpl. 
+unfold blk_term_id. simpl. destruct blk_term. simpl.
+destruct t.
+  +admit.
+  +unfold ssrbool.is_left. destruct (i == pt). simpl. destruct s. constructor; constructor; auto.
+    -destruct f. simpl. constructor. constructor. constructor. right. apply CIH.
+destruct (find_instr blk_code pt i). destruct p. simpl. destruct c. destruct o.
+destruct (i1 == i). simpl. destruct pt. destruct i0.
+simpl. destruct (eval_op e None op). simpl. constructor. constructor.
+simpl. constructor. left. pfold.
+
+
+
+
+
+
+assert (  (memD mem
+     (trace_map (fun _ : state => ())
+        (step_sem
+           {|
+           m_name := m_name;
+           m_target := m_target;
+           m_datalayout := m_datalayout;
+           m_globals := m_globals;
+           m_declarations := m_declarations;
+           m_definitions := m_definitions |}
+           ({| fn := fn; bk := bk; pt := i1 |}, add_env id v e, s))))
+= unroll   (memD mem
+     (trace_map (fun _ : state => ())
+        (step_sem
+           {|
+           m_name := m_name;
+           m_target := m_target;
+           m_datalayout := m_datalayout;
+           m_globals := m_globals;
+           m_declarations := m_declarations;
+           m_definitions := m_definitions |}
+           ({| fn := fn; bk := bk; pt := i1 |}, add_env id v e, s))))).
+destruct ( (memD mem
+     (trace_map (fun _ : state => ())
+        (step_sem
+           {|
+           m_name := m_name;
+           m_target := m_target;
+           m_datalayout := m_datalayout;
+           m_globals := m_globals;
+           m_declarations := m_declarations;
+           m_definitions := m_definitions |}
+           ({| fn := fn; bk := bk; pt := i1 |}, add_env id v e, s))))); auto.
+rewrite H. clear H.
+
+
+assert (  (memD mem
+     (trace_map (fun _ : state => ())
+        (step_sem
+           (optimise_program
+              {|
+              m_name := m_name;
+              m_target := m_target;
+              m_datalayout := m_datalayout;
+              m_globals := m_globals;
+              m_declarations := m_declarations;
+              m_definitions := m_definitions |})
+           ({|
+            fn := fn;
+            bk := bk;
+            pt := get_first_unused
+                    {|
+                    blk_id := blk_id;
+                    blk_phis := blk_phis;
+                    blk_code := blk_code;
+                    blk_term := (i, TERM_Ret_void) |} |},
+           add_env id v e, s))))
+= unroll   (memD mem
+     (trace_map (fun _ : state => ())
+        (step_sem
+           (optimise_program
+              {|
+              m_name := m_name;
+              m_target := m_target;
+              m_datalayout := m_datalayout;
+              m_globals := m_globals;
+              m_declarations := m_declarations;
+              m_definitions := m_definitions |})
+           ({|
+            fn := fn;
+            bk := bk;
+            pt := get_first_unused
+                    {|
+                    blk_id := blk_id;
+                    blk_phis := blk_phis;
+                    blk_code := blk_code;
+                    blk_term := (i, TERM_Ret_void) |} |},
+           add_env id v e, s))))).
+
+destruct   (memD mem
+     (trace_map (fun _ : state => ())
+        (step_sem
+           (optimise_program
+              {|
+              m_name := m_name;
+              m_target := m_target;
+              m_datalayout := m_datalayout;
+              m_globals := m_globals;
+              m_declarations := m_declarations;
+              m_definitions := m_definitions |})
+           ({|
+            fn := fn;
+            bk := bk;
+            pt := get_first_unused
+                    {|
+                    blk_id := blk_id;
+                    blk_phis := blk_phis;
+                    blk_code := blk_code;
+                    blk_term := (i, TERM_Ret_void) |} |},
+           add_env id v e, s)))); auto.
+rewrite H. clear H. subst. unfold get_first_unused. simpl.
+
+
+
+
+
+
+
+
+
+
+
+
+
+
+*)
+
+
+
+
+
+
+
+
+
+
+Admitted.
+
+(*
+(*TERM_RET*)
+
+  +unfold block_to_cmd. simpl. unfold blk_term_id. simpl.
+destruct (i == pt); try_finish. destruct v; simpl.
+destruct (eval_op e (Some t) v); try_finish.
+destruct s; try_finish.
+destruct f. constructor. right. apply CIH. try_finish. 
+destruct (find_instr blk_code pt i); try_finish.
+destruct p; simpl. destruct c.
+    *admit. (*match o*)
+    *destruct t; try_finish.
+      +destruct v0. simpl. destruct (eval_op e (Some t) v0); try_finish. destruct s; try_finish. destruct f. constructor; right; apply CIH. try_finish.
+      +destruct s; try_finish. destruct f. try_finish. constructor. right. apply CIH.
+      +destruct v0. simpl. destruct (eval_op e (Some t) v0); try_finish. destruct v1; try_finish. destruct (StepSemantics.Int1.eq x StepSemantics.Int1.one).
+(*Jump*) admit. (*jump*) admit.
+      +(*Jump*) admit.
+
+(*TERM_RET_VOID*)
+  +unfold block_to_cmd. simpl. unfold blk_term_id. simpl. unfold ssrbool.is_left. destruct (i == pt); try_finish.
+    *destruct s; try_finish. destruct f. try_finish. constructor. right. apply CIH.
+    *destruct (find_instr blk_code pt i); try_finish. destruct p; try_finish. destruct c.
+      -simpl. (*match o*) admit.
+      -simpl. (*one side no instruction*) admit.
+      -simpl. (*one side no instruction *) admit.
+
+
+
+
+(*TERM_BR*)
+  +unfold block_to_cmd. simpl. unfold blk_term_id. simpl. destruct (i == pt). 
+    *simpl. destruct v. simpl. destruct (eval_op e (Some t) v); try_finish. destruct v0; try_finish.
+destruct (StepSemantics.Int1.eq x StepSemantics.Int1.one).
+      -simpl. (*jump*) admit.
+      -simpl. (*jump*) admit.
+    *simpl. destruct (find_instr blk_code pt i).
+      -destruct p. simpl. destruct c.
+        *simpl. (*match o*) admit.
+        *destruct t; try_finish.
+           +destruct v0. simpl. destruct (eval_op e (Some t) v0); try_finish. destruct s; try_finish. destruct f. constructor. right. apply CIH. try_finish.
+           +destruct s; try_finish. destruct f. try_finish. constructor; right; apply CIH.
+           +destruct v0. destruct (eval_op e (Some t) v0); try_finish. destruct v1; try_finish.
+destruct (StepSemantics.Int1.eq x StepSemantics.Int1.one).
+                -simpl. simpl. (*jump*) admit.
+                -simpl. (*jump*) admit.
+        *simpl. (*jump*) admit.
+        *try_finish.
+
+
+(*TERM_BR_1*)
+  +unfold block_to_cmd. simpl. unfold blk_term_id. simpl.
+destruct (i == pt).
+    *simpl. (*jump*) admit.
+    *simpl. destruct (find_instr blk_code pt i); try_finish. destruct p. simpl. destruct c.
+      -simpl. (*match o*) admit.
+      -destruct t; try_finish.
+        +destruct v. simpl. destruct (eval_op e (Some t) v); try_finish. destruct s; try_finish. destruct f. constructor; right; apply CIH. try_finish.
+destruct s; try_finish. destruct f. try_finish. constructor; right; apply CIH.
+        +destruct v. simpl. destruct (eval_op e (Some t) v); try_finish. destruct v0; try_finish. destruct (StepSemantics.Int1.eq x StepSemantics.Int1.one).
+          *simpl. (*jump*) admit.
+          *simpl. (*jump*) admit.
+
+        +(*jump*) admit.
+
+
+(*TERM_SWITCH*)
+  +unfold block_to_cmd. simpl. unfold blk_term_id. simpl. destruct (i == pt); try_finish. destruct (find_instr blk_code pt i).
+    *simpl. destruct p. simpl. destruct c.
+      -simpl. (*match o*) admit.
+      -destruct t; try_finish.
+        +destruct v0. destruct (eval_op e (Some t) v0); try_finish. destruct s; try_finish. destruct f. constructor; right; apply CIH. try_finish.
+destruct s; try_finish. destruct f. try_finish. constructor; right; apply CIH.
+        +destruct v0. simpl. destruct (eval_op e (Some t) v0); try_finish. destruct v1; try_finish. destruct (StepSemantics.Int1.eq x StepSemantics.Int1.one).
+simpl. (*jump*) admit. simpl. (*jump*) admit. (*jump*) admit. try_finish.
+
+(*TERM_INDIRECTBR*)
+
+  +unfold block_to_cmd. simpl. unfold blk_term_id. simpl.
+destruct (i == pt); try_finish. simpl. destruct (find_instr blk_code pt i); try_finish.
+destruct p; simpl. destruct c.
+    *(*match 0*) admit.
+    *destruct t; try_finish.
+      +destruct v0. simpl. destruct (eval_op e (Some t) v0); try_finish. destruct s; try_finish. destruct f. constructor. right. apply CIH. try_finish.
+      +destruct s; try_finish. destruct f. try_finish. constructor. right. apply CIH.
+      +destruct v0. destruct (eval_op e (Some t) v0); try_finish. destruct v1; try_finish. (*jump*) admit.
+      +(*jump *)admit.
+
+
+(*TERM_RESUME*)
+  +unfold block_to_cmd. simpl. unfold blk_term_id. simpl.
+destruct (i == pt); try_finish. simpl. destruct (find_instr blk_code pt i); try_finish.
+destruct p; simpl. destruct c.
+    *(*match o*)admit.
+    *destruct t; try_finish.
+      +destruct v0. simpl. destruct (eval_op e (Some t) v0); try_finish. destruct s; try_finish. destruct f. constructor. right. apply CIH. try_finish.
+      +destruct s; try_finish. destruct f. try_finish. constructor. right. apply CIH.
+      +destruct v0. simpl. destruct (eval_op e (Some t) v0); try_finish. destruct v1; try_finish. (*jump*) admit.
+      +(*jump*) admit.
+
+
+
+(*TERM_INVOKE*)
+  +unfold block_to_cmd. simpl. unfold blk_term_id. simpl.
+destruct (i == pt); try_finish.
+    -simpl. destruct (find_instr blk_code pt i); try_finish. destruct p.
+simpl. destruct c.
+      *simpl. destruct o. unfold ssrbool.is_left. simpl. destruct (i1 == i). simpl. induction pt.
+         +induction i0.
+            -destruct (eval_op e None op). simpl. try_finish.
+                *simpl. admit.
+
+
+
+
+
+
+
+
+
+
+
+
+
+
+
+
+
+
+
+
+
+
+
+
+
+
+
+
+
+
+
+
+
+
+
+
+
+
+
+
+
+
+
+
+
+
+
+                *destruct fn0. destruct i0. simpl. admit.
+                *try_finish.
+                *simpl. 
+constructor. left.
+assert ( (memD (mem ++ [undef])
+     (trace_map (fun _ : state => ())
+        (step_sem prog
+           ({| fn := fn; bk := bk; pt := i1 |},
+           add_env id (DVALUE_Addr (Datatypes.length mem)) e, s)))) = 
+unroll  (memD (mem ++ [undef])
+     (trace_map (fun _ : state => ())
+        (step_sem prog
+           ({| fn := fn; bk := bk; pt := i1 |},
+           add_env id (DVALUE_Addr (Datatypes.length mem)) e, s))))).
+destruct  (memD (mem ++ [undef])
+     (trace_map (fun _ : state => ())
+        (step_sem prog
+           ({| fn := fn; bk := bk; pt := i1 |},
+           add_env id (DVALUE_Addr (Datatypes.length mem)) e, s)))); auto. rewrite H.
+clear H. 
+assert (  (memD (mem ++ [undef])
+     (trace_map (fun _ : state => ())
+        (step_sem (optimise_program prog)
+           ({|
+            fn := fn;
+            bk := bk;
+            pt := get_first_unused
+                    {|
+                    blk_id := blk_id;
+                    blk_phis := blk_phis;
+                    blk_code := blk_code;
+                    blk_term := (i,
+                                TERM_Invoke fnptrval args to_label
+                                  unwind_label) |} |},
+           add_env id (DVALUE_Addr (Datatypes.length mem)) e, s)))) =
+unroll  (memD (mem ++ [undef])
+     (trace_map (fun _ : state => ())
+        (step_sem (optimise_program prog)
+           ({|
+            fn := fn;
+            bk := bk;
+            pt := get_first_unused
+                    {|
+                    blk_id := blk_id;
+                    blk_phis := blk_phis;
+                    blk_code := blk_code;
+                    blk_term := (i,
+                                TERM_Invoke fnptrval args to_label
+                                  unwind_label) |} |},
+           add_env id (DVALUE_Addr (Datatypes.length mem)) e, s))))).
+destruct (  (memD (mem ++ [undef])
+     (trace_map (fun _ : state => ())
+        (step_sem (optimise_program prog)
+           ({|
+            fn := fn;
+            bk := bk;
+            pt := get_first_unused
+                    {|
+                    blk_id := blk_id;
+                    blk_phis := blk_phis;
+                    blk_code := blk_code;
+                    blk_term := (i,
+                                TERM_Invoke fnptrval args to_label
+                                  unwind_label) |} |},
+           add_env id (DVALUE_Addr (Datatypes.length mem)) e, s))))); auto.
+rewrite H.  clear H.
+
+
+
+
+
+
+
+
+
+
+
+
+
+
+
+
+(*simulation*) admit.
+                *destruct ptr. destruct (eval_op e (Some t0) v); simpl.
+                *try_finish.
+                *destruct v0. try_finish. try_finish. 
+                *simpl. (*simulation*) admit.
+                *try_finish.
+                *try_finish.
+                *try_finish.
+                *try_finish.
+                *try_finish.
+                *try_finish.
+                *try_finish.
+                *try_finish.
+                *try_finish.
+                *try_finish.
+                *try_finish.
+                *destruct i0.
+                *try_finish.
+                *destruct fn0. destruct i0. simpl. admit. try_finish. try_finish.  try_finish.
+                *destruct val, ptr. destruct (eval_op e (Some t) v); simpl. try_finish. destruct (eval_op e (Some t0) v0).
+simpl. try_finish. simpl. destruct v2. try_finish. try_finish. (*simulation*) admit. try_finish. try_finish.
+try_finish. try_finish. try_finish. try_finish. try_finish. try_finish. try_finish. try_finish. simpl.
+destruct pt. destruct i0. destruct (eval_op e None op). simpl. try_finish. simpl. constructor. right. apply CIH.
+destruct fn0.  destruct i0. simpl. admit. try_finish. simpl. constructor. right. apply CIH. simpl.
+destruct ptr. destruct (eval_op e (Some t0) v). simpl. try_finish. try_finish. destruct v0.
+try_finish. try_finish. simpl. constructor. right. apply CIH. try_finish. try_finish. try_finish.
+try_finish. try_finish. try_finish. try_finish. try_finish. try_finish. try_finish. try_finish.
+destruct i0. try_finish. destruct fn0. destruct i0. admit. try_finish. try_finish. try_finish.
+destruct val, ptr. simpl. destruct (eval_op e (Some t) v). try_finish. simpl. destruct (eval_op e (Some t0) v0).
+try_finish. try_finish. destruct v2. try_finish. try_finish. admit. try_finish. try_finish. try_finish. try_finish. try_finish.
+try_finish. try_finish. try_finish. try_finish. try_finish. try_finish.
+      *destruct t; try_finish.
+        +destruct v. simpl. destruct (eval_op e (Some t) v); try_finish. destruct s; try_finish. destruct f. constructor. right. apply CIH. try_finish.
+        +destruct s; try_finish. destruct f. simpl. try_finish. constructor. right. apply CIH.
+        +destruct v. simpl. destruct (eval_op e (Some t) v); try_finish. destruct v0; try_finish. admit. (*jump*)
+        +admit.
+ Admitted.*)
+*) Admitted. *) *)*) Admitted.
