src/coq/optimisations/donothing.v
@@ -46,35 +46,81 @@ end.
 Definition test1 prog v args k := unroll_effects ((trace_map (fun _ : state => ()) <$>
    effects_map (step_sem prog) (Call v args k))).
 
+Ltac test X :=
+repeat match goal with
+  | [ |- trace_equiv_step (upaco2 (trace_equiv_step (X:=())) _) (Vis (trace_map (fun _ : state => ()) <$> Err _)) (Vis (trace_map (fun _ : state => ()) <$> Err _)) ] => constructor; constructor
+  | [ |- related_event_step (upaco2 (trace_equiv_step (X:=())) _) (Vis (trace_map (fun _ : state => ()) <$> Err _)) (Vis (trace_map (fun _ : state => ()) <$> Err _)) ] => constructor
+  | [ |- trace_equiv_step (upaco2 (trace_equiv_step (X:=())) _) (Vis (trace_map (fun _ : state => ()) <$> Fin _)) (Vis (trace_map (fun _ : state => ()) <$> Fin _)) ] => constructor; constructor; auto
+  | [ |- trace_equiv_step (upaco2 (trace_equiv_step (X:=())) _) (Tau () (memD _ (trace_map (fun _ : state => ()) (step_sem _ _)))) (Tau () (memD _ (trace_map (fun _ : state => ()) (step_sem _ _))))] => constructor; right; apply X
+
+end.
+
+Ltac destr_simpl P X:= destruct P; simpl; test X.
+
+
 
 
 
 Lemma do_nothing_correct : forall mem st prog, trace_equiv (memD mem (sem prog st)) (memD mem (sem prog st)).
-Proof. Admitted.
-
-
-(*
-(*Initialise*)
-pcofix CIH.
-(*Normal proof.*)
+Proof. pcofix CIH.
 intros. pfold.
-
-(*Unroll left & right function once*)
 assert ((memD mem (sem prog st)) = unroll (memD mem (sem prog st))).
 destruct (memD mem (sem prog st)); eauto. rewrite H. simpl. clear H.
+unfold stepD.
+destruct st.
+destruct p.
+destruct p.
+simpl.
+unfold CFG.fetch.
 
-unfold stepD. destruct st. destruct p. simpl.
-destruct prog. simpl. induction m_definitions.
-  +unfold CFG.fetch. simpl. destruct p. simpl. constructor. constructor.
-  +unfold CFG.fetch in *. simpl in *. destruct p. unfold CFG.find_function in *; simpl in *.
-unfold CFG.find_defn in *; simpl in *. destruct a. simpl in *.
-destruct df_instrs. induction blks.
-destruct (AstLib.ident_of
-                     {|
-                     df_prototype := df_prototype;
-                     df_args := df_args;
-                     df_instrs := {| CFG.init := init; CFG.blks := []; CFG.glbl := glbl |} |} ==
-                   ID_Global fn).
-simpl. constructor. constructor.
+destr_simpl (CFG.find_function prog fn) CIH.
+destr_simpl d CIH. 
+destr_simpl df_instrs CIH.
+destr_simpl (CFG.find_block blks bk) CIH.
+destr_simpl (CFG.block_to_cmd b pt) CIH.
+destr_simpl p CIH.
+destr_simpl c CIH.
+destr_simpl o CIH.
+destr_simpl pt CIH.
+destr_simpl i CIH.
+destr_simpl (eval_op e None op) CIH.
+destr_simpl fn0 CIH.
+destr_simpl i CIH.
+destr_simpl (map_monad (fun '(t0, op) => eval_op e (Some t0) op) args) CIH.
+destr_simpl ((CFG.find_function_entry prog id0)) CIH.
+destr_simpl f CIH.
+destr_simpl (CFG.find_function_entry prog id0) CIH.
+destr_simpl f CIH.
+destr_simpl ptr CIH.
+destr_simpl (eval_op e (Some t0) v) CIH.
+destr_simpl v0 CIH.
+destr_simpl i CIH.
+destr_simpl fn0 CIH.
+destr_simpl i CIH.
+destr_simpl (CFG.find_function_entry prog id) CIH.
+destr_simpl f CIH.
+destr_simpl (map_monad (fun '(t0, op) => eval_op e (Some t0) op) args) CIH.
+destr_simpl t CIH.
+destr_simpl val CIH.
+destr_simpl ptr CIH.
+destr_simpl (eval_op e (Some t) v) CIH.
+destr_simpl (eval_op e (Some t0) v0) CIH.
+destr_simpl v2 CIH.
+destr_simpl t CIH.
+destr_simpl v CIH.
+destr_simpl (eval_op e (Some t) v) CIH.
+destr_simpl s CIH.
+destr_simpl f CIH.
+destr_simpl s CIH.
+destr_simpl f CIH.
+destr_simpl v CIH.
+destr_simpl (eval_op e (Some t) v) CIH.
+destr_simpl v0 CIH.
+destr_simpl (StepSemantics.Int1.eq x StepSemantics.Int1.one) CIH.
+destr_simpl (jump prog fn bk br1 e s) CIH.
+destr_simpl (jump prog fn bk br2 e s) CIH.
+destr_simpl (jump prog fn bk br e s) CIH.
+Qed.
 
-*)
+
+
