src/coq/optimisations/paco_util.v
@@ -2,7 +2,14 @@ Require Import paco.
 Require Import Vellvm.Effects.
 Require Import Vellvm.StepSemantics.
 Require Import Vellvm.Ollvm_ast.
+Require Import Vellvm.Memory.
+Require Import Vellvm.Effects.
+Require Import ZArith List String Omega.
+Require Import  Vellvm.Ollvm_ast Vellvm.Classes Vellvm.Util Vellvm.CFGProp Vellvm.CFG.
 
+
+Set Implicit Arguments.
+Set Contextual Implicit.
 
 Module A : Vellvm.StepSemantics.ADDR with Definition addr := nat.
   Definition addr := nat.
@@ -11,23 +18,13 @@ End A.
 Module SS := StepSemantics.StepSemantics(A).
 Export SS.
 
+Ltac finish X :=
+repeat match goal with
+  | [ |- trace_equiv_step (upaco2 (trace_equiv_step (X:=())) _) (Vis (trace_map (fun _ : state => ()) <$> Err _)) (Vis (trace_map (fun _ : state => ()) <$> Err _)) ] => constructor; constructor
+  | [ |- related_event_step (upaco2 (trace_equiv_step (X:=())) _) (Vis (trace_map (fun _ : state => ()) <$> Err _)) (Vis (trace_map (fun _ : state => ()) <$> Err _)) ] => constructor
+  | [ |- trace_equiv_step (upaco2 (trace_equiv_step (X:=())) _) (Vis (trace_map (fun _ : state => ()) <$> Fin _)) (Vis (trace_map (fun _ : state => ()) <$> Fin _)) ] => constructor; constructor; auto
+  | [ |- trace_equiv_step (upaco2 (trace_equiv_step (X:=())) _) (Tau () (memD _ (trace_map (fun _ : state => ()) (step_sem _ _)))) (Tau () (memD _ (trace_map (fun _ : state => ()) (step_sem _ _))))] => constructor; right; apply X
 
-    Module ET : Vellvm.Effects.EffT
-        with Definition addr := A.addr
-        with Definition typ := Ollvm_ast.typ
-        with Definition value := dvalue.
+end.
 
-      Definition addr := A.addr.
-      Definition typ := Ollvm_ast.typ.
-      Definition value := dvalue.
-      Definition inj_addr := DVALUE_Addr.
-      Definition no_value := DV (VALUE_None).
-    End ET.    
-  Module E := Vellvm.Effects.Effects(ET).
-  Export E.
-
-
-
-
-
-
+Ltac destr_simpl P X:= destruct P; simpl; finish X.
